rename_ctx_preserv_types

label-free/Semantics.v
@@ -11,66 +11,79 @@ Open Scope label_free_is5_scope.
 Global Reserved Notation " G '|=' Ctx '|-' M ':::' A " (at level 70).
  
 (* Statics *)
-
-Fixpoint ok_Bg (G: Background_LF) (Used: list var) : Prop :=
-match G with
+Fixpoint ok A (G: list (var * A)) (Used: list var) : Prop :=
+match G with 
 | nil => True
-| (w, Gamma) :: G' => 
-    If (Mem w Used) then False 
-    else ok_Bg G' (w::Used)
+| (w, Gamma) :: G => If Mem w Used then False else ok A G (w::Used)
 end.
+
+Definition ok_Bg (G: Background_LF) : Prop :=
+ok (list (var * ty_LF)) G nil  /\
+ok (ty_LF) (flat_map snd G) nil.
 
 Inductive types_LF: Background_LF -> Context_LF -> te_LF -> ty_LF -> Prop :=
 
-| t_hyp_LF: forall A G w Gamma v_n
-  (HT: Nth v_n Gamma A),
-  G |= (w, Gamma) |- hyp_LF v_n ::: A
+| t_hyp_LF: forall A G w Gamma v
+  (Ok_Bg: ok_Bg ((w, Gamma) :: G))
+  (HT: Mem (v, A) Gamma),
+  G |= (w, Gamma) |- hyp_LF (fvar v) ::: A
 
-| t_lam_LF: forall A B G w Gamma M
-  (HT: G |= (w, A::Gamma) |- M ::: B),
+| t_lam_LF: forall L A B G w Gamma M
+  (Ok_Bg: ok_Bg ((w, Gamma) :: G))
+  (HT: forall v', v' \notin L -> 
+    G |= (w, (v', A) :: Gamma) |- M ^t^ (hyp_LF (fvar v')) ::: B),
   G |= (w, Gamma) |- (lam_LF A M) ::: A ---> B
 
-| t_appl_LF: forall A B G Ctx M N
-  (HT1: G |= Ctx |- M ::: A ---> B)
-  (HT2: G |= Ctx |- N ::: A),
-  G |= Ctx |- (appl_LF M N) ::: B
+| t_appl_LF: forall A B G w Gamma M N
+  (Ok_Bg: ok_Bg ((w, Gamma) :: G))
+  (HT1: G |= (w, Gamma) |- M ::: A ---> B)
+  (HT2: G |= (w, Gamma) |- N ::: A),
+  G |= (w, Gamma) |- (appl_LF M N) ::: B
 
-| t_box_LF: forall L A G Ctx M
+| t_box_LF: forall L A G w Gamma M
+  (Ok_Bg: ok_Bg (G & (w, Gamma)))
   (HT: forall w', w' \notin L -> 
-    G & Ctx |= (w', nil) |- M ^^ [fctx w' | fctx w'] ::: A),
-  G |= Ctx |- box_LF M ::: [*] A
+    G & (w, Gamma) |= (w', nil) |- M ^w^ (fctx w') ::: A),
+  G |= (w, Gamma) |- box_LF M ::: [*] A
 
 | t_unbox_LF: forall A G w Gamma M
+  (Ok_Bg: ok_Bg ((w, Gamma) :: G))
   (HT: G |= (w, Gamma) |- M ::: [*] A),
   G |= (w, Gamma) |- unbox_fetch_LF (fctx w) M ::: A
 
-| t_unbox_fetch_LF: forall A G w Gamma Ctx' M
-  (HT: G & Ctx' |= (w, Gamma) |- M ::: [*] A),
+| t_unbox_fetch_LF: forall A G w Gamma w' Gamma' M
+  (Ok_Bg: ok_Bg ((w, Gamma) :: G & (w', Gamma')))
+  (HT: (G & (w', Gamma')) |= (w, Gamma) |- M ::: [*] A),
   forall G', permut (G & (w, Gamma)) G' ->
-    G' |= Ctx' |- unbox_fetch_LF (fctx w) M ::: A
+    G' |= (w', Gamma') |- unbox_fetch_LF (fctx w) M ::: A
 
 | t_here_LF: forall A G w Gamma M
+  (Ok_Bg: ok_Bg ((w, Gamma) :: G))
   (HT: G |= (w, Gamma) |- M ::: A),
   G |= (w, Gamma) |- get_here_LF (fctx w) M ::: <*> A
 
 | t_get_here_LF: forall A G w Gamma Ctx' M
+  (Ok_Bg: ok_Bg ((w, Gamma) :: G & Ctx'))
   (HT: G & Ctx' |= (w, Gamma) |- M ::: A),
   forall G', permut (G & (w, Gamma)) G' -> 
     G' |= Ctx' |- get_here_LF (fctx w) M ::: <*> A
 
-| t_letdia_LF: forall L A B G w Gamma M N
+| t_letdia_LF: forall L_w L_t A B G w Gamma M N
+  (Ok_Bg: ok_Bg ((w, Gamma) :: G))
   (HT1: G |= (w, Gamma) |- M ::: <*> A)
-  (HT2: forall w', w' \notin L ->
-    (w', A :: nil) :: G |= (w, Gamma) |- N ^^ [fctx w' | fctx w] ::: B),
+  (HT2: forall v', v' \notin L_t -> forall w', w' \notin L_w ->
+    (w', (v', A) :: nil) :: G |= 
+      (w, Gamma) |- (N ^w^ (fctx w')) ^t^ (hyp_LF (fvar v')) ::: B),
   G |= (w, Gamma) |- letdia_get_LF (fctx w) M N ::: B 
 
-| t_letdia_get_LF: forall L A B G w Gamma Ctx' M N
+| t_letdia_get_LF: forall L_w L_t A B G w Gamma Ctx' M N
+  (Ok_Bg: ok_Bg ((w, Gamma) :: G & Ctx'))
   (HT1: G & Ctx' |= (w, Gamma) |- M ::: <*> A)
-  (HT2: forall w', w' \notin L ->
-    (w', (A :: nil)) :: G & (w, Gamma) |= Ctx' |- N ^^ [fctx w' | fctx (fst Ctx')] ::: B),
+  (HT2: forall v', v' \notin L_t -> forall w', w' \notin L_w ->
+    (w', ((v', A) :: nil)) :: G & (w, Gamma) |= 
+      Ctx' |- (N ^w^ (fctx w')) ^t^ (hyp_LF (fvar v')) ::: B),
   forall G0, permut (G & (w, Gamma)) G0 -> 
     G0 |= Ctx' |- letdia_get_LF (fctx w) M N ::: B
-
 where " G '|=' Ctx '|-' M ':::' A " := (types_LF G Ctx M A) : label_free_is5_scope.
 
 (* Dynamics *)
@@ -85,1830 +98,44 @@ Global Reserved Notation " M |-> N " (at level 70).
 
 Inductive step_LF: (te_LF * ctx_LF) -> (te_LF * ctx_LF) -> Prop :=
 | red_appl_lam_LF: forall ctx M A N,
-  lc_w_LF M -> lc_w_LF N ->
-  (appl_LF (lam_LF A M) N, ctx) |-> 
-    ([N // 0 | ctx ] [M | ctx], ctx)
+  lc_w_LF M -> lc_t_n_LF M 1 ->
+  lc_w_LF N -> lc_t_LF N ->
+  (appl_LF (lam_LF A M) N, ctx) |-> ( M ^t^ N , ctx)
 
 | red_unbox_fetch_box_LF: forall ctx ctx' M,
-  lc_w_n_LF M 1 ->
-  (unbox_fetch_LF ctx' (box_LF M), ctx) |-> 
-    (M ^^ [ctx | ctx], ctx) 
+  lc_w_n_LF M 1 -> lc_t_LF M ->
+  (unbox_fetch_LF ctx' (box_LF M), ctx) |-> (M ^w^ ctx, ctx)
 
 | red_letdia_get_get_here_LF: forall ctx ctx' ctx'' M N,
-  lc_w_LF M ->
-  lc_w_n_LF N 1 ->
-  (letdia_get_LF ctx' (get_here_LF ctx'' M) N, ctx) |-> 
-    ([M // 0 | ctx'' ] [N ^^ [ctx'' | ctx] | ctx] , ctx)
+  lc_w_LF M -> lc_t_LF M ->
+  lc_w_n_LF N 1 -> lc_t_n_LF N 1 ->
+  (letdia_get_LF ctx' (get_here_LF ctx'' M) N, ctx) |-> ((N ^w^ ctx'') ^t^ M, ctx)
 
 | red_appl_LF: forall ctx M N M'
   (HT: (M, ctx) |-> (M', ctx)), 
-  lc_w_LF M ->
-  lc_w_LF N ->
+  lc_w_LF M -> lc_t_LF M ->
+  lc_w_LF N -> lc_t_LF N ->
   (appl_LF M N, ctx) |-> (appl_LF M' N, ctx)
 
 | red_unbox_fetch_LF: forall ctx' M M' ctx
   (HT: (M, ctx') |-> (M', ctx')), 
-  lc_w_n_LF M 1 ->
+  lc_w_LF M -> lc_t_LF M ->
   (unbox_fetch_LF ctx' M, ctx) |-> (unbox_fetch_LF ctx' M', ctx)
 
 | red_get_here_LF: forall ctx ctx' M M' 
   (HT: (M, ctx) |-> (M', ctx)), 
-  lc_w_LF M ->
+  lc_w_LF M -> lc_t_LF M ->
   (get_here_LF ctx M, ctx') |-> (get_here_LF ctx M', ctx')
 
 | red_letdia_get_LF: forall ctx ctx' M N M'
   (HT: (M, ctx) |-> (M', ctx)), 
-  lc_w_LF M ->
-  lc_w_n_LF N 1->
+  lc_w_LF M -> lc_t_LF M ->
+  lc_w_n_LF N 1 -> lc_t_n_LF N 1 ->
   (letdia_get_LF ctx M N, ctx') |-> (letdia_get_LF ctx M' N, ctx')
 
 where " M |-> N " := (step_LF M N ) : label_free_is5_scope.
 
-(* Extensions to tlc library *)
-
-Section PermutationAdd.
-Variable A: Type.
-Implicit Type l : list A.
-
-Lemma permut_inv:
-forall G0 G0' G1 G1' (elem: A),
-  permut (G0 & elem ++ G0') (G1 & elem ++ G1') ->
-  permut (G0 ++ G0') (G1 ++ G1').
-Admitted.
-
-Lemma permut_split_neq:
-forall G G' H (elem:A) (elem':A)
-  (HNeq: elem <> elem')
-  (HT: permut (G & elem ++ G') (H & elem')),
-  exists GH, exists GT, H = GH & elem ++ GT.
-Admitted.
-
-(* TODO: Reconsider Permutation from standard library and / or make permut a Setoid *)
-(* TODO: Move the extended permutation lib to a separate file *)
-
-End PermutationAdd.
-
 Section Lemmas.
-
-Lemma BackgroundSubsetImpl:
-forall G G' Ctx M A
-  (HT: G |= Ctx |- M ::: A)
-  (HSubst: exists GT, permut (G++GT) G'),
-  G' |= Ctx |- M ::: A.
-intros;
-generalize dependent G';
-induction HT; intros; eauto using types_LF.
-(* box *)
-destruct HSubst as [GT];
-apply t_box_LF with (L:=L); intros;
-apply H; [ | exists GT; permut_simpl]; assumption.
-(* unbox_fetch *)
-destruct HSubst as [GT];
-apply t_unbox_fetch_LF with (Gamma:=Gamma) (G:=G++GT);
-[ apply IHHT; exists GT; permut_simpl | 
-  apply permut_trans with (l2:= G' ++ GT)]; 
-[ permut_simpl | ]; assumption.
-(* get_here *)
-destruct HSubst as [GT];
-apply t_get_here_LF with (Gamma:=Gamma) (G:=G++GT);
-[ apply IHHT; exists GT; permut_simpl |
-  apply permut_trans with (l2:= G' ++ GT)]; 
-[ permut_simpl | ]; assumption.
-(* letdia *)
-apply t_letdia_LF with (A:=A) (L:=L);
-[ apply IHHT; assumption | 
-  intros; apply H]; 
-auto;
-destruct HSubst as [GT];
-exists GT; permut_simpl; assumption.
-(* letdia_get *)
-destruct HSubst as [GT];
-apply t_letdia_get_LF with (A:=A) (Gamma:=Gamma) (G:=G++GT) (L:=L);
-[ apply IHHT; exists GT; permut_simpl | 
-  intros; apply H | 
-  apply permut_trans with (l2:= G0 ++ GT) ];
-auto;
-[ exists GT |
-  apply permut_trans with (l2:= G0 ++ GT)];
-permut_simpl; auto.
-Qed.
-
-Lemma GlobalWeakening:
-forall G G' Ctx Ctx' M A
-  (HT: G ++ G' |= Ctx |- M ::: A),
-  G & Ctx' ++ G' |= Ctx |- M ::: A.
-intros; rew_app;
-apply BackgroundSubsetImpl with (G := G ++ G');
-[assumption | exists (Ctx'::nil)];
-permut_simpl.
-Qed.
-
-Lemma Weakening_general:
-  forall G w Gamma M A
-  (HT: G |= (w, Gamma) |- M ::: A),
-  (forall G' w' Delta Delta',
-    permut G (G' & (w', Delta)) ->
-    G' & (w', Delta ++ Delta') |= (w, Gamma) |- M ::: A) /\ 
-  (forall Gamma',
-    G |= (w, Gamma ++ Gamma') |- M ::: A).
-intros;
-remember (w, Gamma) as Ctx;
-generalize dependent Gamma;
-generalize dependent w;
-induction HT; split;
-intros; subst; simpl;
-try (inversion HeqCtx; subst).
-(* hyp *)
-eauto using types_LF.
-constructor; generalize dependent v_n;
-induction Gamma0; destruct v_n; intros;
-try (apply Nth_nil_inv in HT; contradiction);
-apply Nth_app_l; assumption.
-(* lam *)
-constructor; eapply IHHT; eauto.
-constructor;
-apply IHHT with (w:=w0) (Gamma:=A::Gamma0);
-auto.
-(* appl *)
-econstructor; [eapply IHHT1| eapply IHHT2]; eauto.
-econstructor; [eapply IHHT1| eapply IHHT2]; eauto.
-(* box 1 *)
-apply t_box_LF with (L:=L); intros;
-apply BackgroundSubsetImpl with (G:=G' & (w, Gamma) & (w', Delta ++ Delta')).
-  eapply H; eauto.
-    apply permut_trans with (l2:=G' & (w', Delta) & (w, Gamma)).
-      apply permut_app_lr; auto.
-      permut_simpl. 
-  exists (@nil Context_LF); permut_simpl; assumption.
-(* box 2 *)
-apply t_box_LF with (L:=L); intros;
-eapply H; eauto; permut_simpl.
-(* unbox *)
-constructor; eapply IHHT; eauto.
-constructor; eapply IHHT; eauto.
-(* unbox_fetch 1 *)
-destruct (eq_context_LF_dec (w', Delta) (w, Gamma)).
-(* = *)
-inversion e; subst;
-apply t_unbox_fetch_LF with (G:=G) (Gamma:=Gamma++Delta');
-[ apply IHHT; reflexivity | 
-  permut_simpl];
-replace G with (G++nil) by (rew_app; reflexivity);
-replace G'0 with (G'0++nil) by (rew_app; reflexivity);
-apply permut_inv with (elem := (w, Gamma));
-apply permut_trans with (l2:=G'); permut_simpl; assumption.
-(* <> *)
-assert (exists G0, exists G1, G'0 = G0 & (w, Gamma) ++ G1).
-  apply permut_split_neq with (G:=G) (G':=nil) (elem':=(w',Delta)).
-    intro e; symmetry in e; contradiction.
-    rew_app; apply permut_trans with (l2:=G'); assumption.
-destruct H1 as [GH]; destruct H1 as [GT]; subst G'0.
-apply t_unbox_fetch_LF with (Gamma:=Gamma) (G:=GH ++ GT & (w', Delta ++ Delta')).
-apply BackgroundSubsetImpl with (G:= (GH ++ GT & (w0, Gamma0)) & (w', Delta ++ Delta')).
-  specialize IHHT with w Gamma.  
-  destruct IHHT; try reflexivity.
-  apply H1 with (G':= GH ++ GT & (w0, Gamma0)).
-  permut_simpl.
-  assert (permut (G++nil) (GH ++ GT & (w', Delta))).
-    apply permut_inv with (elem := (w ,Gamma)).
-    apply permut_trans with (l2:=G').
-    rew_app; assumption.
-    apply permut_trans with (l2:=(GH & (w, Gamma) ++ GT) & (w', Delta)).
-      assumption.
-      permut_simpl.
-  rew_app in H3.
-  apply permut_app_l with (l2:=(w0, Gamma0)::nil) in H3.
-  apply permut_trans with (l2:=(GH ++ GT & (w', Delta) & (w0, Gamma0))).
-    rew_app in *. assumption.
-    permut_simpl.
-  exists (@nil Context_LF); permut_simpl.
-permut_simpl.
-(* unbox_fetch 2 *)
-apply t_unbox_fetch_LF with (G:=G) (Gamma:=Gamma).
-  specialize IHHT with w Gamma.
-destruct IHHT; try reflexivity.
-apply H0.
-permut_simpl.
-assumption.
-(* here *)
-constructor; specialize IHHT with w0 Gamma0; apply IHHT; auto. 
-constructor; apply IHHT; auto.
-(* get_here 1 *)
-destruct (eq_context_LF_dec (w', Delta) (w, Gamma)).
-(* = *)
-inversion e;
-subst;
-apply t_get_here_LF with (Gamma:=Gamma++Delta') (G:=G).
-  apply IHHT.
-  reflexivity.
-  apply permut_app_l.
-  assert (permut (G & (w, Gamma)) (G'0 & (w, Gamma))).
-  apply permut_trans with (l2:=G'); assumption.
-  replace G with (G++nil) by (rew_app; reflexivity).
-  replace G'0 with (G'0++nil) by (rew_app; reflexivity).
-  apply permut_inv with (elem:=(w, Gamma)).
-  rew_app; assumption.
-(* <> *)
-assert (exists G0, exists G1, G'0 = G0 & (w, Gamma) ++ G1).
-  apply permut_split_neq with (G:=G) (G':=nil) (elem':=(w', Delta)).
-    intro e; symmetry in e; contradiction.
-    rew_app; apply permut_trans with (l2:=G'); assumption.
-destruct H1 as [GH]; destruct H1 as [GT]; subst G'0.
-apply t_get_here_LF with (Gamma:=Gamma) (G:=GH ++ GT & (w', Delta ++ Delta')).
-apply BackgroundSubsetImpl with (G:= (GH ++ GT & (w0, Gamma0)) & (w', Delta ++ Delta')).
-  specialize IHHT with w Gamma.
-  apply IHHT. 
-  reflexivity.
-  assert (permut (G++nil) (GH++GT & (w', Delta))).
-    apply permut_inv with (elem := (w ,Gamma)).
-    apply permut_trans with (l2:=G').
-    rew_app; assumption.
-    apply permut_trans with (l2:=(GH & (w, Gamma) ++ GT) & (w', Delta)).
-      assumption.
-      permut_simpl.
-  rew_app in H1.
-  apply permut_app_l with (l2:=(w0,Gamma0)::nil) in H1.
-  apply permut_trans with (l2:=(GH ++ GT & (w', Delta)) & (w0, Gamma0)).
-    assumption.
-    permut_simpl.
-  exists (@nil Context_LF); permut_simpl.
-  permut_simpl.
-(* get_here 2 *)
-apply t_get_here_LF with (G:=G) (Gamma:=Gamma).
-  specialize IHHT with w Gamma.
-  apply IHHT. 
-    reflexivity.
-    permut_simpl.
-  assumption.
-(* letdia *)
-apply t_letdia_LF with (A:=A) (L:=L).
-specialize IHHT with w0 Gamma0.
-apply IHHT; auto.
-intros. 
-specialize H with (w':=w'0).
-destruct H with (w:=w0) (Gamma:=Gamma0).
-assumption.
-reflexivity.
-apply H2 with (G':=(w'0, A::nil)::G');
-permut_simpl;
-assumption.
-apply t_letdia_LF with (A:=A) (L:=L).
-apply IHHT; auto.
-intros; apply H; auto.
-(* letdia_get 1 *)
-destruct (eq_context_LF_dec (w', Delta) (w, Gamma)).
-(* = *)
-inversion e;
-subst;
-apply t_letdia_get_LF with (Gamma:=Gamma++Delta') (G:=G) (A:=A) (L:=L).
-  apply IHHT.
-  reflexivity.
-  intros.
-  specialize H with (w':=w').
-  destruct H with (w1:=w0)(Gamma1:=Gamma0).
-    assumption.
-    reflexivity.
-  apply H3 with (G':= (w', A :: nil) :: G).
-  permut_simpl.
-  apply permut_app_l.
-  assert (permut (G & (w, Gamma)) (G' & (w, Gamma))).
-  apply permut_trans with (l2:=G0); assumption.
-  replace G with (G++nil) by (rew_app; reflexivity).
-  replace G' with (G'++nil) by (rew_app; reflexivity).
-  apply permut_inv with (elem:=(w, Gamma)).
-  rew_app; assumption.
-(* <> *)
-assert (exists G0, exists G1, G' = G0 & (w, Gamma) ++ G1).
-  apply permut_split_neq with (G:=G) (G':=nil) (elem':=(w', Delta)).
-    intro e; symmetry in e; contradiction.
-    rew_app; apply permut_trans with (l2:=G0); assumption.
-destruct H2 as [GH]; destruct H2 as [GT]; subst G'.
-apply t_letdia_get_LF with (Gamma:=Gamma) (G:=GH ++ GT & (w', Delta ++ Delta')) (L:=L)(A:=A).
-apply BackgroundSubsetImpl with (G:= (GH ++ GT & (w0, Gamma0)) & (w', Delta ++ Delta')).
-  specialize IHHT with w Gamma.
-  apply IHHT. 
-  reflexivity.
-  assert (permut (G++nil) (GH++GT & (w', Delta))).
-    apply permut_inv with (elem := (w ,Gamma)).
-    apply permut_trans with (l2:=G0).
-    rew_app; assumption.
-    apply permut_trans with (l2:=(GH & (w, Gamma) ++ GT) & (w', Delta)).
-      assumption.
-      permut_simpl.
-  rew_app in H2.
-  apply permut_app_l with (l2:=(w0,Gamma0)::nil) in H2.
-  apply permut_trans with (l2:=(GH ++ GT & (w', Delta)) & (w0, Gamma0)).
-    assumption.
-    permut_simpl.
-  exists (@nil Context_LF); permut_simpl.
-  intros.
-  specialize H with (w':=w'0).
-  destruct H with (w1:=w0) (Gamma1:=Gamma0).
-    assumption.
-    reflexivity.
-  apply BackgroundSubsetImpl with (G:=((w'0, A::nil) :: GH++GT &(w, Gamma)) & (w', Delta ++ Delta')).
-  apply H3.
-  permut_simpl.
-  assert (permut (G & (w, Gamma)) (GH ++ GT & (w', Delta) & (w, Gamma) )).
-    apply permut_trans with (l2:= (GH & (w,Gamma) ++ GT) & (w', Delta)).
-      apply permut_trans with (l2:=G0); assumption.
-    permut_simpl.
-  replace G with (G++nil) by (rew_app; reflexivity).
-  replace (GH++GT & (w',Delta)) with ((GH++GT & (w',Delta))++nil) by (rew_app; reflexivity).
-  apply permut_inv with (elem := (w, Gamma)). 
-  rew_app in *; assumption.
-exists (@nil Context_LF); permut_simpl.
-permut_simpl.
-(* letdia_get 2 *)
-apply t_letdia_get_LF with (G:=G) (Gamma:=Gamma) (A:=A) (L:=L).
-  specialize IHHT with w Gamma.
-  apply IHHT. 
-    reflexivity.
-    permut_simpl.
-  intros.
-  specialize H with (w':=w'); destruct H with (w1:=w0)(Gamma1:=Gamma0).
-  assumption.
-  reflexivity.
-  apply H3.
-  assumption.
-Qed.
-
-Lemma WeakeningBackgroundElem:
-forall G G' w Delta Delta' Ctx M A
-  (HT: G & (w, Delta) ++ G' |= Ctx |- M ::: A),
-  G & (w, Delta ++ Delta') ++ G' |= Ctx |- M ::: A.
-intros;
-apply BackgroundSubsetImpl with (G:=(G++G') & (w, Delta ++ Delta')).
-assert (permut (G & (w, Delta) ++ G') ((G++G') & (w, Delta))) by  permut_simpl;
-destruct Ctx;
-eapply Weakening_general; eassumption.
-eexists nil; permut_simpl.
-Qed.
-
-Lemma Weakening:
-forall G w Gamma Gamma' M A
-  (HT: G |= (w, Gamma) |- M ::: A),
-  G |= (w, Gamma ++ Gamma') |- M ::: A.
-intros;
-eapply Weakening_general; eassumption.
-Qed.
-
-(* Original formulations of modified typing rules can be reconstructed *)
-Lemma test_box:
-  forall L G G' Ctx M A,
-    (forall w', w' \notin L -> 
-      G & Ctx ++ G' |=  (w', nil) |- M^^[fctx w' | fctx w'] ::: A) ->
-      G ++ G' |= Ctx |- box_LF M ::: [*]A.
-intros; apply t_box_LF with (L:=L); intros;
-try assumption;
-apply BackgroundSubsetImpl with (G:=G & Ctx ++ G');
-[ apply H; assumption
-|  exists (@nil Context_LF); permut_simpl].
-Qed.
-
-Lemma test_unbox_fetch:
-  forall G G' Ctx w' Gamma' M A,
-    G & Ctx ++ G' |= (w', Gamma') |- M ::: [*] A ->
-      G & (w', Gamma') ++ G' |= Ctx |- unbox_fetch_LF (fctx w') M ::: A.
-intros;
-apply t_unbox_fetch_LF with (G:=G ++ G') (Gamma:=Gamma');
-[apply BackgroundSubsetImpl with (G:=G & Ctx ++ G') | permut_simpl];
-[ assumption | exists (@nil Context_LF); permut_simpl].
-Qed.
-
-Lemma test_get_here:
-  forall G G' Ctx w' Gamma' M A,
-    G & Ctx ++ G' |= (w', Gamma') |- M ::: A ->
-      G & (w', Gamma') ++ G' |= Ctx |- get_here_LF (fctx w') M ::: <*> A.
-intros;
-apply t_get_here_LF with (G:=G ++ G') (Gamma:=Gamma');
-[apply BackgroundSubsetImpl with (G:=G & Ctx ++ G') | permut_simpl];
-[assumption | exists (@nil Context_LF); permut_simpl].
-Qed.
-
-Lemma test_letdia_get:
-  forall L G G' w w' Gamma Gamma' M N A B,
-    G & (w', Gamma') ++ G' |= (w, Gamma) |- M ::: <*>A ->
-    (forall w'', w'' \notin L -> 
-      (w'', (A::nil)) :: G & (w, Gamma) ++ G' |= (w', Gamma') 
-        |- N ^^ [fctx w'' | fctx w'] ::: B) ->
-    G & (w, Gamma) ++ G' |= (w', Gamma') |-  letdia_get_LF (fctx w) M N ::: B.
-intros;
-apply t_letdia_get_LF with (A:=A) (G:=G ++ G') (L:=L) (Gamma := Gamma); intros;
-[ apply BackgroundSubsetImpl with (G:=G & (w', Gamma') ++ G') |
-  apply BackgroundSubsetImpl with (G:=(w'0, A::nil) :: G & (w, Gamma) ++ G') |
-  permut_simpl];
-  [assumption | exists (@nil Context_LF); permut_simpl |
-   apply H0; assumption | exists (@nil Context_LF); permut_simpl ].
-Qed.
-
-(* / *)
-
-(* emptyEquiv = map (fun x => (x, nil)) (map fst G) *)
-Fixpoint emptyEquiv (G: Background_LF) : Background_LF :=
-match G with
-| nil => nil
-| (w, a)::G => (w, nil) :: emptyEquiv G
-end.
-
-Lemma emptyEquiv_nil:
-forall G G' w Gamma,
-  permut (emptyEquiv G) G' ->
-  Mem (w, Gamma) G' -> Gamma = nil.
-Admitted.
-
-Lemma emptyEquiv_empty:
-forall G G',
-  permut (emptyEquiv G) G' ->
-  emptyEquiv G' = G'.
-Admitted.
-
-Lemma emptyEquiv_inv:
-forall G G' w,
-  emptyEquiv (G & (w,nil)) = (G' & (w, nil)) ->
-  emptyEquiv G = G'.
-Admitted.
-
-Lemma emptyEquiv_last:
-forall G G' Gamma w,
-  emptyEquiv G = G' ->
-  emptyEquiv (G & (w, Gamma)) = G' & (w, nil).
-Admitted.
-
-Lemma emptyEquiv_stable:
-forall G,
-  emptyEquiv (emptyEquiv G) = emptyEquiv G.
-Admitted.
-
-Lemma emptyEquiv_permut:
-forall G G',
-  permut G G' ->
-  permut (emptyEquiv G) (emptyEquiv G').
-Admitted.
-
-Lemma emptyEquiv_typing:
-forall G w Gamma M A
-  (HT: emptyEquiv G |= (w, Gamma) |- M ::: A),
-  G |= (w, Gamma) |- M ::: A.
-Admitted.
-
-Lemma emptyEquiv_dom:
-forall G,
-  map fst G = map fst (emptyEquiv G).
-Admitted.
-
-(* TODO: get rid of this, using ok_Bg instead should work! *)
-Lemma unique_worlds:
-forall G G' w w' Gamma Gamma' M A
-  (HPermut: permut G' (G & (w', Gamma')))
-  (HT: G' |= (w, Gamma) |- M ::: A),
-  w <> w'.
-Admitted.
-
-Lemma Nth_last:
-forall Gamma (A: ty_LF) A',
-  Nth (length Gamma) (Gamma & A) A' -> A = A'.
-Admitted.
-
-Lemma Nth_not_last:
-forall Gamma (A: ty_LF) A' n,
-  Nth n (Gamma & A) A' ->
-  n <> length Gamma ->
-  Nth n Gamma A'.
-Admitted.
-
-(* TODO: It's not really smart yet.. *)
-(* Goal of smart destruct is to destruct chains of assumptions without loosing
-   any of them; it should also work when the chain is conditional, but the
-   condition is easily checked to be true (e.g. provable by reflexivity) *)
-Ltac smart_destruct :=
-match goal with
-| [H: ?w = ?w -> _ |- _] => destruct H; [reflexivity | try smart_destruct]
-| [H: ?w = ?w -> ?w' = ?w' -> _ |- _] => 
-  destruct H; [reflexivity | reflexivity | try smart_destruct]
-| [H: ?t1 = ?t2 /\ _ |- _] => destruct H; try smart_destruct 
-end.
-
-Lemma ok_Bg_permut:
-forall G G' L,
-  permut  G G' ->
-  ok_Bg G L -> ok_Bg G' L.
-Admitted.
-
-Lemma ok_Bg_change_last:
-forall G w Gamma Gamma' L,
-  ok_Bg (G & (w, Gamma)) L ->
-  ok_Bg (G & (w, Gamma')) L.
-Admitted.
-
-Lemma ok_Bg_emptyEquiv:
-forall G L,
-  ok_Bg G L = ok_Bg (emptyEquiv G) L.
-Admitted.
-
-(* TODO: add_fresh and add_new are too specialized and should be 
-         removed (or changed) *)
-Lemma ok_Bg_add_fresh:
-forall G w Gamma w' Gamma' L,
-  w' \notin (\{w} \u from_list (map fst G) \u from_list L) ->
-  ok_Bg ((w, Gamma)::G) L ->
-  ok_Bg ((w', Gamma') :: (w, Gamma) :: G) L. 
-Admitted.
-
-Lemma ok_Bg_add_new:
-forall G w Gamma L,
-  w \notin from_list(map fst G) ->
-  ok_Bg G L ->
-  ok_Bg ((w, Gamma) :: G) L.
-Admitted.
-
-Lemma ok_Bg_unify:
-forall G G0 G1 w Gamma Gamma',
-  permut G (G0 & (w, Gamma)) ->
-  permut G (G1 & (w, Gamma')) ->
-  ok_Bg G nil ->
-  Gamma = Gamma'.
-Admitted.
-
-Lemma ok_Bg_step:
-forall G L w,
-  ok_Bg G (w::L) ->
-  ok_Bg G L.
-Admitted.
-
-Lemma ok_Bg_swap:
-forall G w Gamma Gamma' L,
-  ok_Bg (G & (w, Gamma)) L ->
-  ok_Bg ((w, Gamma')::G) L.
-Admitted.
-
-Lemma emptyEquiv_mem:
-forall G G' w,
-  permut (emptyEquiv G) (emptyEquiv G') ->
-  w \notin from_list (map fst G) -> 
-  w \notin from_list (map fst G').
-Admitted.
-
-Fixpoint subst_typing G L D w : Prop :=
-match L, D with
-| nil, nil => True
-| M::L', A :: D' => emptyEquiv G |= (w, nil) |- M ::: A /\ (subst_typing G L' D' w)
-| _, _ => False
-end.
-
-Ltac try_rewrite_subst :=
-try repeat rewrite subst_t__inner;
-try repeat erewrite subst_t__outer;
-try repeat rewrite subst_ctx__new;
-try repeat rewrite subst_ctx__old;
-try repeat rewrite subst_ctx__outer; 
-eauto.
-
-Lemma subst_t_preserv_types_end:
-forall G_HT w Gamma_HT M N B
-  (H_lc: lc_w_LF M)
-  (H_G_ok: ok_Bg ((w, Gamma_HT) :: G_HT) nil)
-  (HT: G_HT |= (w, Gamma_HT) |- N ::: B),
-  forall A Gamma_TS w_subst G_min Gamma_subst G_TS G0,
-  ( emptyEquiv G_HT |= (w, nil) |- M ::: A ->
-    Gamma_HT = Gamma_TS & A ->
-    G_HT |= (w, Gamma_TS) |- [ M // length Gamma_TS | fctx w] [ N | fctx w ] ::: B)
-  /\
-  ( permut G_min (G0 & (w, Gamma_HT)) ->
-    permut G_HT (G0 & (w_subst, Gamma_subst & A)) ->
-    permut G_TS (G0 & (w_subst, Gamma_subst)) -> 
-    w_subst <> w ->
-    ok_Bg ((w_subst, nil)::G_min) nil -> 
-    ok_Bg ((w, Gamma_HT) :: G_TS) nil ->
-    emptyEquiv G_min |= (w_subst, nil) |- M ::: A ->
-    G_TS |= (w, Gamma_HT) |- [ M // length Gamma_subst | fctx w_subst] [ N | fctx w ] ::: B).
-intros until A;
-remember (w, Gamma_HT) as Ctx_HT;
-generalize dependent Gamma_HT;
-generalize dependent w;
-generalize dependent A;
-induction HT; intros; split; 
-inversion HeqCtx_HT;
-subst; unfold subst_t; intros;
-case_if; simpl; subst.
-
-(* hyp inner *)
-case_if; subst.
-(* v_n = length Gamma *)
-apply Nth_last in HT; subst;
-replace Gamma_TS with (nil ++ Gamma_TS) by auto;
-apply Weakening;
-apply emptyEquiv_typing in H; assumption.
-(* v_n <> length Gamma *)
-constructor;
-generalize dependent v_n;
-induction Gamma_TS; simpl in *; intros.
-(* nil *)
-rew_length in H0;
-destruct v_n;
-[ elim H0; reflexivity | 
-  inversion HT; subst]; 
-apply Nth_nil_inv in H6; contradiction.
-(* step *)
-destruct v_n; simpl in *;
-inversion HT; subst;
-eapply Nth_not_last;
-eassumption.
-
-(* hyp outer *)
-constructor; assumption.
-
-(* lam inner *)
-constructor; subst;
-replace (S (length Gamma_TS)) with (length (A0 :: Gamma_TS)) by (rew_length; omega);
-rewrite subst_t__inner;
-eapply IHHT with (Gamma_TS := A::Gamma_TS); eauto.
-
-(* lam outer *)
-constructor; subst;
-rewrite subst_t__outer with (w':=fctx w0); auto;
-eapply IHHT; eauto.
-replace ((w_subst, nil) :: G0 & (w0, A :: Gamma_HT)) with 
-        (((w_subst, nil) :: G0) & (w0, A :: Gamma_HT)) by (rew_app; reflexivity).
-apply ok_Bg_change_last with (Gamma:= Gamma_HT).
-apply ok_Bg_permut with (G := (w_subst, nil)::G_min); try permut_simpl; auto.
-apply emptyEquiv_permut in H;
-rewrite emptyEquiv_last with (G':=emptyEquiv G0) in H; auto.
-rewrite emptyEquiv_last with (G':=emptyEquiv G0); auto;
-apply BackgroundSubsetImpl with (G:=emptyEquiv G_min);
-[ | exists (@nil Context_LF); permut_simpl]; auto;
-erewrite <- emptyEquiv_last; eauto;
-eapply emptyEquiv_permut; eauto.
-
-(* appl inner *)
-apply t_appl_LF with (A:=A);
-rewrite subst_t__inner;
-[edestruct IHHT1 | edestruct IHHT2];
-eauto.
-
-(* appl outer *)
-apply t_appl_LF with (A:=A); subst;
-rewrite subst_t__outer with (w':=fctx w); auto;
-[ eapply IHHT1 | 
-  eapply IHHT2 ]; 
-eauto.
-
-(* box inner *)
-apply t_box_LF with (L:=L \u \{w} \u from_list(map fst G)); intros;
-repeat rewrite notin_union in H2; destruct H2 as (H2a, H2b);
-destruct H2b as (H2b, H2c);
-assert (w' <> w) by
- (intro; subst; rewrite notin_singleton in H2b; elim H2b; reflexivity);
-rewrite subst_t__outer with (w':=fctx w'); 
-try (intro nn; inversion nn; subst; elim H2; reflexivity);
-unfold open_ctx in *;
-rewrite <- subst_order_irrelevant; eauto;
-eapply H; eauto.
-
-apply ok_Bg_permut with (G:=(w',nil)::(w, Gamma_TS & A0)::G); try permut_simpl.
-apply ok_Bg_add_fresh;
-[repeat rewrite notin_union; repeat split | ]; auto. apply notin_empty.
-
-simpl. simpl in H_G_ok. case_if.
-apply ok_Bg_permut with (G:=(w',nil)::G). 
-permut_simpl.
-apply ok_Bg_add_new. assumption.
-assumption.
-
-remember ((w',nil)::G) as G_w'.
-assert (ok_Bg (G_w' & (w, Gamma_TS)) nil).
-apply ok_Bg_change_last with (Gamma:=Gamma_TS & A0).
-assert (ok_Bg ((w', nil) :: G & (w, Gamma_TS & A0)) nil).
-apply ok_Bg_permut with (G:=(w',nil)::(w, Gamma_TS & A0)::G); try permut_simpl.
-apply ok_Bg_add_fresh.
-repeat rewrite notin_union; repeat split; try assumption.
-apply notin_empty.
-
-assumption.
-subst; rew_app in *; assumption.
-subst; rew_app in *; assumption.
-
-rewrite emptyEquiv_last with (G':=emptyEquiv G); auto;
-replace (emptyEquiv G & (w', nil)) with (emptyEquiv G & (w', nil) ++ nil) 
-  by (rew_app; reflexivity);
-apply GlobalWeakening; rew_app; assumption.
-
-(* box outer *)
-apply t_box_LF with (L:=L \u \{w_subst} \u \{w} \u from_list (map fst G)); intros;
-apply notin_union in H9; destruct H9;
-apply notin_union in H10; destruct H10;
-apply notin_union in H11; destruct H11;
-rewrite subst_t__outer with (w':=fctx w');
-try (intro nn; inversion nn; subst; elim H8; reflexivity);
-unfold open_ctx in *.
-rewrite <- subst_order_irrelevant; auto;
-assert (permut (G & (w, Gamma_HT)) (G0 & (w, Gamma_HT) & (w_subst, Gamma_subst & A0)))by
-  (permut_simpl; assumption);
-eapply H; eauto.
-
-apply ok_Bg_permut with (G:=(w',nil)::(w, Gamma_HT)::G); try permut_simpl.
-apply ok_Bg_add_fresh;
-[repeat rewrite notin_union; repeat split | ]; try assumption;
-apply notin_empty.
-
-apply permut_trans with (l2:=G0 & (w_subst, Gamma_subst) & (w, Gamma_HT));
-[ apply permut_app_l; assumption | permut_simpl].
-
-rewrite ok_Bg_emptyEquiv.
-apply ok_Bg_permut with (G:=emptyEquiv((w',nil)::(w, Gamma_HT)::G)).
-apply emptyEquiv_permut in H2. 
-simpl; simpl in H2.
-rewrite emptyEquiv_last with (G':=emptyEquiv G0 & (w, nil)).
-rewrite emptyEquiv_last with (G':=emptyEquiv G0) in H2. 
-permut_simpl.
-apply permut_trans with (l2:=emptyEquiv (G0 & (w_subst, Gamma_HT))).
-  rewrite emptyEquiv_last with (G' := emptyEquiv G0).
-  assumption.
-reflexivity.
-  rewrite emptyEquiv_last with (G' := emptyEquiv G0).
-permut_simpl.
-reflexivity.
-reflexivity.
-  rewrite emptyEquiv_last with (G' := emptyEquiv G0).
-  reflexivity.
-  reflexivity.
-rewrite <- ok_Bg_emptyEquiv.
-apply ok_Bg_add_fresh;
-[repeat rewrite notin_union; repeat split | ]; auto.
-apply notin_empty.
-
-rewrite ok_Bg_emptyEquiv.
-apply ok_Bg_permut with (G:=emptyEquiv((w',nil)::(w, Gamma_HT)::G)).
-apply emptyEquiv_permut in H3. 
-simpl; simpl in H3.
-permut_simpl.
-apply permut_trans with (l2:=emptyEquiv (G0 & (w_subst, Gamma_subst) & (w, Gamma_HT))).
-rewrite emptyEquiv_last with (G':=emptyEquiv (G0 & (w_subst, nil))).
-rewrite emptyEquiv_last with (G':=emptyEquiv G0).
-permut_simpl.
-apply emptyEquiv_permut in H2.
-rewrite emptyEquiv_last with (G':=emptyEquiv G0) in H2. 
-assumption.
-reflexivity.
-reflexivity.
-rewrite emptyEquiv_last with (G':=emptyEquiv G0).
-rewrite emptyEquiv_last with (G':=emptyEquiv G0).
-reflexivity.
-reflexivity.
-reflexivity.
-apply permut_sym.
-rewrite emptyEquiv_last with (G':= emptyEquiv G_TS). 
-rewrite emptyEquiv_last with (G':= emptyEquiv (G0 & (w_subst, Gamma_subst))). 
-permut_simpl. assumption.
-reflexivity.
-reflexivity.
-rewrite <- ok_Bg_emptyEquiv.
-apply ok_Bg_add_fresh;
-[repeat rewrite notin_union; repeat split | ]; auto;
-apply notin_empty.
-
-rewrite emptyEquiv_last with (G' := emptyEquiv (G0 & (w, Gamma_HT))); auto;
-replace (emptyEquiv (G0 & (w, Gamma_HT)) & (w', nil)) with (emptyEquiv (G0 & (w, Gamma_HT)) & (w', nil) ++ nil) by (rew_app; auto).
-apply GlobalWeakening; rew_app;
-apply BackgroundSubsetImpl with (G:= emptyEquiv G_min);
-[ assumption | exists (@nil Context_LF)]; 
-permut_simpl; apply emptyEquiv_permut; assumption.
-intro nn; inversion nn; subst. rewrite notin_singleton in H10. elim H10; reflexivity.
-
-(* unbox inner *)
-case_if; constructor; 
-rewrite subst_t__inner;
-eapply IHHT; eauto.
-
-(* unbox outer *)
-case_if;
-constructor;
-rewrite subst_t__outer with (w':=fctx w0); eauto;
-eapply IHHT; eauto.
-
-(* unbox_fetch inner *)
-assert (w0 <> w) by
-  (apply emptyEquiv_permut in H;
-   apply BackgroundSubsetImpl with (G':=emptyEquiv (G & (w, Gamma))) in H1;
-   try rewrite emptyEquiv_last with (G':=emptyEquiv G) in H1; auto;
-   try eapply unique_worlds; eauto;
-   exists (@nil Context_LF); permut_simpl; apply permut_sym; auto);
-case_if;
-apply t_unbox_fetch_LF with (G:=G) (Gamma:=Gamma); auto;
-rewrite subst_t__outer with (w':=fctx w); eauto;
-eapply IHHT; eauto.
-
-apply ok_Bg_permut with (G:=(w0, Gamma_TS & A0) :: G').
-apply permut_trans with (l2:=(w0, Gamma_TS & A0) :: (w,Gamma)::G).
-permut_simpl. apply permut_sym; apply permut_trans with (l2:=G & (w, Gamma)).
-permut_simpl. assumption.
-permut_simpl.
-assumption.
-
-rewrite ok_Bg_emptyEquiv.
-apply ok_Bg_permut with (G:= emptyEquiv ((w0, Gamma_TS & A0) :: G')).
-simpl; permut_simpl; apply emptyEquiv_permut in H. 
-apply permut_sym; assumption.
-rewrite <- ok_Bg_emptyEquiv; assumption.
-
-assert (permut ((w, Gamma)::G & (w0, Gamma_TS & A0)) ((w0, Gamma_TS & A0) :: G')).
-apply permut_trans with (l2:=((w0, Gamma_TS & A0) :: G & (w, Gamma))).
-permut_simpl. permut_simpl; assumption.
-rewrite ok_Bg_emptyEquiv.
-apply ok_Bg_permut with (G:=emptyEquiv ((w0, Gamma_TS & A0) :: G')).
-apply emptyEquiv_permut in H5. apply permut_sym.
-remember ((w, Gamma) :: G) as G_w. 
-assert (permut (emptyEquiv (G_w & (w0, Gamma_TS))) (emptyEquiv ((w0, Gamma_TS & A0) :: G'))).
-rewrite emptyEquiv_last with (G':=emptyEquiv G_w). 
-replace ((w, Gamma) :: G & (w0, Gamma_TS & A0)) with (G_w & (w0, Gamma_TS & A0)) in H5.
-rewrite emptyEquiv_last with (G':=emptyEquiv G_w) in H5. 
-assumption.
-reflexivity.
-subst; rew_app; reflexivity.
-reflexivity.
-subst; rew_app in *; assumption.
-rewrite ok_Bg_emptyEquiv in H_G_ok; assumption.
-
-apply BackgroundSubsetImpl with (G:=emptyEquiv G');
-[ assumption |
-  exists (@nil Context_LF)];
-rew_app; apply emptyEquiv_permut;
-apply permut_sym; assumption.
-
-(* unbox_fetch outer *)
-case_if.
-(* switch back to inner *)
-inversion H9; subst.
-assert (Gamma_subst & A0 = Gamma). 
-apply ok_Bg_unify with (G:=G') (G0:=G0) (G1:= G) (w:=w).
-assumption.
-apply permut_sym; assumption.
-simpl in H_G_ok. rewrite Mem_nil_eq in H_G_ok. case_if.
-apply ok_Bg_step in H_G_ok; assumption.
-subst Gamma.
-
-assert (permut G G0).
-assert (permut (G & (w, Gamma_subst & A0) ++ nil) (G0 & (w, Gamma_subst & A0) ++ nil)).
-rew_app; apply permut_trans with (l2:=G'); assumption.
-apply permut_inv in H10. rew_app in H10; assumption.
-
-apply t_unbox_fetch_LF with (G:=G) (Gamma:=Gamma_subst).
-rewrite subst_t__inner.
-eapply IHHT with (Gamma_TS := Gamma_subst) (Gamma_HT0 := Gamma_subst & A0) (w1 := w) (A1:=A0); eauto.
-
-apply ok_Bg_permut with (G:=(w0, Gamma_HT) :: G').
-apply permut_trans with (l2:=((w0, Gamma_HT)::(w, Gamma_subst & A0) :: G)).
-permut_simpl.
-apply permut_trans with (l2:= (G0 & (w, Gamma_subst & A0))).
-assumption.
-permut_simpl. apply permut_sym; assumption.
-permut_simpl.
-assumption.
-
-apply BackgroundSubsetImpl with (G:=emptyEquiv G_min); eauto.
-exists (@nil Context_LF). 
-apply permut_trans with (l2:=emptyEquiv (G0 & (w0, Gamma_HT))).
-apply emptyEquiv_permut in H1; rew_app; assumption.
-apply emptyEquiv_permut; apply permut_sym; apply permut_app_l; assumption.
-apply permut_trans with (l2:=G0 & (w, Gamma_subst)).
-apply permut_app_l; assumption.
-apply permut_sym; assumption.
-(* stay in outer *)
-assert (exists GH, exists GT, G0 = GH & (w, Gamma) ++ GT).
-apply permut_split_neq with (G:=G) (G':=nil) (elem':=(w_subst, Gamma_subst & A0)).
-intro nn; inversion nn; subst; elim H9; reflexivity.
-apply permut_trans with (l2:=G'). 
-rew_app; assumption.
-assumption.
-
-destruct H10 as [GH]; destruct H10 as [GT].
-apply t_unbox_fetch_LF with (G:=GH++GT & (w_subst, Gamma_subst)) (Gamma:=Gamma).
-rewrite subst_t__outer with (w':= fctx w).
-subst.
-eapply IHHT with (Gamma_subst := Gamma_subst) (w_subst:=w_subst) (w1:=w) (G0:=GH ++ GT & (w0, Gamma_HT)) (G_TS:=(GH++GT & (w_subst, Gamma_subst)) & (w0, Gamma_HT)) (A0:=A0); eauto.
-
-apply ok_Bg_permut with (G:=(w0, Gamma_HT) :: G').
-apply permut_trans with (l2:= (w0, Gamma_HT) :: (G & (w, Gamma))).
-permut_simpl. apply permut_sym; assumption.
-permut_simpl.
-assumption.
-
-apply permut_trans with (l2:=((GH ++ GT & (w_subst, Gamma_subst & A0)) & (w0, Gamma_HT))).
-apply permut_app_l.
-assert (permut (G & (w, Gamma)) ((GH & (w, Gamma) ++ GT) & (w_subst, Gamma_subst & A0))). 
-apply permut_trans with (l2:=G'); assumption.
-replace G with (G++nil).
-replace (GH ++ GT & (w_subst, Gamma_subst & A0)) with (GH ++ GT & (w_subst, Gamma_subst & A0) ++ nil).
-apply permut_inv with (elem:=(w, Gamma)).
-rew_app in *; assumption.
-rew_app; reflexivity.
-rew_app; reflexivity.
-permut_simpl.
-
-permut_simpl.
-intro nn; subst; elim H9; reflexivity.
-
-apply ok_Bg_permut with (G:= (w_subst, nil):: G_min).
-permut_simpl.
-apply permut_trans with (l2:=(GH & (w, Gamma) ++ GT) & (w0, Gamma_HT)).
-assumption.
-permut_simpl.
-assumption.
-
-apply ok_Bg_permut with (G:= (w_subst, Gamma_subst)::G_min).
-permut_simpl.
-apply permut_trans with (l2:=(GH & (w, Gamma) ++ GT) & (w0, Gamma_HT)).
-assumption.
-permut_simpl.
-rewrite ok_Bg_emptyEquiv.
-rewrite ok_Bg_emptyEquiv in H5.
-simpl in *. rewrite Mem_nil_eq in *. case_if.
-assumption.
-
-apply BackgroundSubsetImpl with (G:=emptyEquiv G_min).
-eassumption.
-exists (@nil Context_LF).
-apply permut_trans with (l2:=emptyEquiv ((GH & (w, Gamma) ++ GT) & (w0, Gamma_HT))).
-apply emptyEquiv_permut in H1; rew_app in *; assumption.
-apply emptyEquiv_permut; permut_simpl.
-assumption.
-apply permut_trans with (l2:=G0 & (w_subst, Gamma_subst)).
-subst; permut_simpl.
-apply permut_sym; assumption.
-
-(* here inner *)
-case_if; constructor; 
-rewrite subst_t__inner;
-eapply IHHT; eauto.
-
-(* here outer *)
-case_if; constructor;
-rewrite subst_t__outer with (w':=fctx w0); auto;
-eapply IHHT; eauto.
-
-(* get_here inner *)
-assert (w0 <> w) by
-  (apply emptyEquiv_permut in H;
-   apply BackgroundSubsetImpl with (G':=emptyEquiv (G & (w, Gamma))) in H1;
-   try rewrite emptyEquiv_last with (G':=emptyEquiv G) in H1; auto;
-   try eapply unique_worlds; eauto;
-   exists (@nil Context_LF); permut_simpl; apply permut_sym; auto);
-case_if.
-apply t_get_here_LF with (G:=G) (Gamma:=Gamma); auto;
-rewrite subst_t__outer with (w':=fctx w); eauto;
-eapply IHHT; eauto.
-
-apply ok_Bg_permut with (G:=(w0, Gamma_TS & A0) :: G').
-apply permut_trans with (l2:=(w0, Gamma_TS & A0) :: (w,Gamma)::G).
-permut_simpl. apply permut_sym; apply permut_trans with (l2:=G & (w, Gamma)).
-permut_simpl. assumption.
-permut_simpl.
-assumption.
-
-rewrite ok_Bg_emptyEquiv.
-apply ok_Bg_permut with (G:= emptyEquiv ((w0, Gamma_TS & A0) :: G')).
-simpl; permut_simpl; apply emptyEquiv_permut in H. 
-apply permut_sym; assumption.
-rewrite <- ok_Bg_emptyEquiv; assumption.
-
-assert (permut ((w, Gamma)::G & (w0, Gamma_TS & A0)) ((w0, Gamma_TS & A0) :: G')).
-apply permut_trans with (l2:=((w0, Gamma_TS & A0) :: G & (w, Gamma))).
-permut_simpl. permut_simpl; assumption.
-rewrite ok_Bg_emptyEquiv.
-apply ok_Bg_permut with (G:=emptyEquiv ((w0, Gamma_TS & A0) :: G')).
-apply emptyEquiv_permut in H5. apply permut_sym.
-remember ((w, Gamma) :: G) as G_w. 
-assert (permut (emptyEquiv (G_w & (w0, Gamma_TS))) (emptyEquiv ((w0, Gamma_TS & A0) :: G'))).
-rewrite emptyEquiv_last with (G':=emptyEquiv G_w). 
-replace ((w, Gamma) :: G & (w0, Gamma_TS & A0)) with (G_w & (w0, Gamma_TS & A0)) in H5.
-rewrite emptyEquiv_last with (G':=emptyEquiv G_w) in H5. 
-assumption.
-reflexivity.
-subst; rew_app; reflexivity.
-reflexivity.
-subst; rew_app in *; assumption.
-rewrite ok_Bg_emptyEquiv in H_G_ok; assumption.
-
-apply BackgroundSubsetImpl with (G:=emptyEquiv G');
-[ assumption |
-  exists (@nil Context_LF)];
-rew_app; apply emptyEquiv_permut;
-apply permut_sym; assumption.
-
-(* get_here outer *)
-case_if.
-(* switch back to inner *)
-inversion H9; subst.
-assert (Gamma_subst & A0 = Gamma). 
-apply ok_Bg_unify with (G:=G') (G0:=G0) (G1:= G) (w:=w).
-assumption.
-apply permut_sym; assumption.
-simpl in H_G_ok. rewrite Mem_nil_eq in H_G_ok. case_if.
-apply ok_Bg_step in H_G_ok; assumption.
-subst Gamma.
-
-assert (permut G G0).
-assert (permut (G & (w, Gamma_subst & A0) ++ nil) (G0 & (w, Gamma_subst & A0) ++ nil)).
-rew_app; apply permut_trans with (l2:=G'); assumption.
-apply permut_inv in H10. rew_app in H10; assumption.
-
-apply t_get_here_LF with (G:=G) (Gamma:=Gamma_subst).
-rewrite subst_t__inner.
-eapply IHHT with (Gamma_TS := Gamma_subst) (Gamma_HT0 := Gamma_subst & A0) (w1 := w) (A1:=A0); eauto.
-
-apply ok_Bg_permut with (G:=(w0, Gamma_HT) :: G').
-apply permut_trans with (l2:=((w0, Gamma_HT)::(w, Gamma_subst & A0) :: G)).
-permut_simpl.
-apply permut_trans with (l2:= (G0 & (w, Gamma_subst & A0))).
-assumption.
-permut_simpl. apply permut_sym; assumption.
-permut_simpl.
-assumption.
-
-apply BackgroundSubsetImpl with (G:=emptyEquiv G_min); eauto.
-exists (@nil Context_LF). 
-apply permut_trans with (l2:=emptyEquiv (G0 & (w0, Gamma_HT))).
-apply emptyEquiv_permut in H1; rew_app; assumption.
-apply emptyEquiv_permut; apply permut_sym; apply permut_app_l; assumption.
-apply permut_trans with (l2:=G0 & (w, Gamma_subst)).
-apply permut_app_l; assumption.
-apply permut_sym; assumption.
-(* stay in outer *)
-assert (exists GH, exists GT, G0 = GH & (w, Gamma) ++ GT).
-apply permut_split_neq with (G:=G) (G':=nil) (elem':=(w_subst, Gamma_subst & A0)).
-intro nn; inversion nn; subst; elim H9; reflexivity.
-apply permut_trans with (l2:=G'). 
-rew_app; assumption.
-assumption.
-
-destruct H10 as [GH]; destruct H10 as [GT].
-apply t_get_here_LF with (G:=GH++GT & (w_subst, Gamma_subst)) (Gamma:=Gamma).
-rewrite subst_t__outer with (w':= fctx w).
-subst.
-eapply IHHT with (Gamma_subst := Gamma_subst) (w_subst:=w_subst) (w1:=w) (G0:=GH ++ GT & (w0, Gamma_HT)) (G_TS:=(GH++GT & (w_subst, Gamma_subst)) & (w0, Gamma_HT)) (A0:=A0); eauto.
-
-apply ok_Bg_permut with (G:=(w0, Gamma_HT) :: G').
-apply permut_trans with (l2:= (w0, Gamma_HT) :: (G & (w, Gamma))).
-permut_simpl. apply permut_sym; assumption.
-permut_simpl.
-assumption.
-
-apply permut_trans with (l2:=((GH ++ GT & (w_subst, Gamma_subst & A0)) & (w0, Gamma_HT))).
-apply permut_app_l.
-assert (permut (G & (w, Gamma)) ((GH & (w, Gamma) ++ GT) & (w_subst, Gamma_subst & A0))). 
-apply permut_trans with (l2:=G'); assumption.
-replace G with (G++nil).
-replace (GH ++ GT & (w_subst, Gamma_subst & A0)) with (GH ++ GT & (w_subst, Gamma_subst & A0) ++ nil).
-apply permut_inv with (elem:=(w, Gamma)).
-rew_app in *; assumption.
-rew_app; reflexivity.
-rew_app; reflexivity.
-permut_simpl.
-
-permut_simpl.
-intro nn; subst; elim H9; reflexivity.
-
-apply ok_Bg_permut with (G:= (w_subst, nil):: G_min).
-permut_simpl.
-apply permut_trans with (l2:=(GH & (w, Gamma) ++ GT) & (w0, Gamma_HT)).
-assumption.
-permut_simpl.
-assumption.
-
-apply ok_Bg_permut with (G:= (w_subst, Gamma_subst)::G_min).
-permut_simpl.
-apply permut_trans with (l2:=(GH & (w, Gamma) ++ GT) & (w0, Gamma_HT)).
-assumption.
-permut_simpl.
-rewrite ok_Bg_emptyEquiv.
-rewrite ok_Bg_emptyEquiv in H5.
-simpl in *. rewrite Mem_nil_eq in *. case_if.
-assumption.
-
-apply BackgroundSubsetImpl with (G:=emptyEquiv G_min).
-eassumption.
-exists (@nil Context_LF).
-apply permut_trans with (l2:=emptyEquiv ((GH & (w, Gamma) ++ GT) & (w0, Gamma_HT))).
-apply emptyEquiv_permut in H1; rew_app in *; assumption.
-apply emptyEquiv_permut; permut_simpl.
-assumption.
-apply permut_trans with (l2:=G0 & (w_subst, Gamma_subst)).
-subst; permut_simpl.
-apply permut_sym; assumption.
-
-(* letdia inner *)
-case_if; apply t_letdia_LF with (L:=L \u \{w0} \u from_list (map fst G)) (A:=A);
-rewrite subst_t__inner.
-eapply IHHT; eauto.
-intros.
-unfold open_ctx.
-rewrite <- subst_order_irrelevant; eauto.
-eapply H; eauto.
-apply ok_Bg_permut with (G:= (w', A::nil) :: ((w0, Gamma_TS & A0)::G)).
-permut_simpl.
-apply ok_Bg_add_fresh.
-repeat rewrite notin_union in *; destruct H3. destruct H4.
-repeat split; auto; apply notin_empty.
-assumption.
-
-replace ( emptyEquiv ((w', A :: nil) :: G)) with (nil & (w', nil) ++ emptyEquiv G).
-apply GlobalWeakening; rew_app; assumption.
-simpl; rew_app; reflexivity. 
-
-(* letdia outer *)
-case_if; apply t_letdia_LF 
-  with (L:=L \u \{w0} \u from_list (map fst G) \u \{w_subst}) (A:=A).
-
-rewrite subst_t__outer with (w':=fctx w0); eauto;
-eapply IHHT; eauto.
-
-intros;
-rewrite subst_t__outer with (w':=fctx w0); auto.
-unfold open_ctx;
-rewrite <- subst_order_irrelevant; eauto.
-eapply H with (G_TS := (w', A::nil) :: G_TS) (G0:=(w', A::nil) :: G0) ; eauto.
-
-apply ok_Bg_permut with (G:=(w', A::nil) :: ((w0,Gamma_HT) :: G)).
-permut_simpl.
-apply ok_Bg_add_fresh.
-repeat rewrite notin_union in *;
-destruct H9; destruct H10; destruct H11.
-repeat split; try assumption. apply notin_empty.
-assumption.
-
-permut_simpl; eassumption.
-permut_simpl; assumption.
-
-rewrite ok_Bg_emptyEquiv.
-apply ok_Bg_permut with (G := (w', nil):: (w0,nil) :: emptyEquiv G).
-apply permut_trans with (l2:=emptyEquiv((w', nil) :: (w0, nil)::G0 & (w_subst, Gamma_subst & A0))).
-permut_simpl.
-simpl. permut_simpl. apply emptyEquiv_permut in H1; assumption.
-permut_simpl. simpl. permut_simpl.
-rewrite emptyEquiv_last with (G':=emptyEquiv G0).
-rewrite emptyEquiv_last with (G':=emptyEquiv G0).
-permut_simpl.
-reflexivity. 
-reflexivity.
-apply ok_Bg_add_fresh.
-repeat rewrite notin_union in *;
-destruct H9; destruct H10; destruct H11.
-repeat split. assumption.
-rewrite <- emptyEquiv_dom. assumption.
-apply notin_empty.
-replace ((w0,nil)::emptyEquiv G) with (emptyEquiv ((w0,nil)::G)) by (simpl; reflexivity).
-apply ok_Bg_permut with (G:=emptyEquiv ((w0, Gamma_HT)::G_TS)).
-simpl. permut_simpl.
-apply permut_trans with (l2:=emptyEquiv G0 & (w_subst, nil)).
-replace (emptyEquiv G0 & (w_subst, nil)) with (emptyEquiv (G0 & (w_subst, Gamma_subst))).
-apply emptyEquiv_permut. assumption.
-replace (emptyEquiv G0 & (w_subst, nil)) with (emptyEquiv (G0 & (w_subst, Gamma_subst & A0))).
-rewrite emptyEquiv_last with (G':=emptyEquiv G0).
-rewrite emptyEquiv_last with (G':=emptyEquiv G0).
-reflexivity.
-reflexivity.
-reflexivity.
-rewrite emptyEquiv_last with (G':=emptyEquiv G0).
-reflexivity.
-reflexivity.
-replace (emptyEquiv G0 & (w_subst, nil)) with (emptyEquiv (G0 & (w_subst, Gamma_subst & A0))).
-apply emptyEquiv_permut in H1; apply permut_sym. assumption.
-rewrite emptyEquiv_last with (G':=emptyEquiv G0).
-reflexivity.
-reflexivity.
-rewrite <- ok_Bg_emptyEquiv. assumption.
-
-apply ok_Bg_permut with (G:=(w', A::nil)::(w0, Gamma_HT)::G_TS).
-permut_simpl.
-apply ok_Bg_add_fresh.
-repeat rewrite notin_union in *;
-destruct H9; destruct H10; destruct H11.
-repeat split. assumption.
-apply emptyEquiv_mem with (G:=G).
-apply permut_trans with (l2:=emptyEquiv (G0 & (w_subst, Gamma_subst))).
-rewrite emptyEquiv_last with (G':=emptyEquiv G0).
-apply emptyEquiv_permut in H1.
-rewrite emptyEquiv_last with (G':=emptyEquiv G0) in H1.
-assumption.
-reflexivity.
-reflexivity.
-apply emptyEquiv_permut in H2. apply permut_sym; assumption.
-assumption.
-apply notin_empty.
-assumption.
-
-apply BackgroundSubsetImpl with (G:=emptyEquiv G_min).
-assumption.
-exists ((w',(@nil ty_LF))::nil); permut_simpl; simpl;
-permut_simpl.
-apply emptyEquiv_permut; assumption.
-
-(* letdia_get inner *)
-assert (w0 <> w) by
-  (apply emptyEquiv_permut in H0;
-   apply BackgroundSubsetImpl with (G':=emptyEquiv (G & (w, Gamma))) in H2;
-   try rewrite emptyEquiv_last with (G':=emptyEquiv G) in H2; auto;
-   try eapply unique_worlds; eauto;
-   exists (@nil Context_LF); permut_simpl; apply permut_sym; auto);
-case_if.
-eapply t_letdia_get_LF with (L:=L \u \{w0} \u \{w} \u from_list(map fst G)); eauto.
-rewrite subst_t__outer with (w':= fctx w).
-eapply IHHT; eauto.
-
-apply ok_Bg_permut with (G:=(w0, Gamma_TS & A0) :: G0).
-apply permut_trans with (l2:= (w0, Gamma_TS & A0) :: G & (w, Gamma)).
-permut_simpl.
-apply permut_sym; assumption.
-permut_simpl.
-assumption.
-
-apply ok_Bg_permut with ((w0, nil)::G0).
-permut_simpl; apply permut_sym; assumption.
-rewrite ok_Bg_emptyEquiv in H_G_ok; 
-rewrite ok_Bg_emptyEquiv.
-simpl in *; assumption. 
-
-apply ok_Bg_permut with ((w0, Gamma_TS)::G0).
-apply permut_trans with (l2:=(w0, Gamma_TS)::G & (w, Gamma)).
-permut_simpl. apply permut_sym. assumption.
-permut_simpl.
-assumption.
-
-apply BackgroundSubsetImpl with (G:=emptyEquiv G0).
-assumption.
-exists (@nil Context_LF); rew_app; apply emptyEquiv_permut. apply permut_sym; assumption.
-assumption.
-
-intros.
-rewrite subst_t__inner.
-unfold open_ctx; rewrite <- subst_order_irrelevant; auto.
-eapply H; eauto.
-
-apply ok_Bg_permut with (G:=(w', A::nil)::(w0, Gamma_TS & A0) :: (w, Gamma) :: G).
-permut_simpl.
-apply ok_Bg_add_fresh.
-repeat rewrite notin_union in *.
-destruct H6; destruct H7; destruct H8.
-split. assumption.
-rewrite map_cons. simpl.
-rewrite from_list_cons.
-repeat rewrite notin_union; repeat split; auto. apply notin_empty.
-apply ok_Bg_permut with (G:=(w0, Gamma_TS & A0) :: G0).
-permut_simpl.
-apply permut_trans with (l2:=G & (w, Gamma)).
-apply permut_sym; assumption.
-permut_simpl.
-assumption.
-
-simpl.
-replace ((w', nil) :: emptyEquiv (G & (w, Gamma))) with (nil & (w', nil) ++ emptyEquiv (G & (w, Gamma))).
-apply GlobalWeakening; rew_app.
-apply BackgroundSubsetImpl with (G:=emptyEquiv G0).
-assumption.
-exists (@nil Context_LF).
-rew_app; apply emptyEquiv_permut.
-apply permut_sym; assumption.
-rew_app; reflexivity.
-
-(* letdia_get outer *)
-case_if.
-(* switch back to inner *)
-inversion H10; subst.
-assert (Gamma_subst & A0 = Gamma). 
-apply ok_Bg_unify with (G:=G0) (G0:=G1) (G1:= G) (w:=w).
-assumption.
-apply permut_sym; assumption.
-simpl in H_G_ok. rewrite Mem_nil_eq in H_G_ok. case_if.
-apply ok_Bg_step in H_G_ok; assumption.
-subst Gamma.
-
-assert (permut G G1).
-assert (permut (G & (w, Gamma_subst & A0) ++ nil) (G1 & (w, Gamma_subst & A0) ++ nil)).
-rew_app; apply permut_trans with (l2:=G0); assumption.
-apply permut_inv in H11. rew_app in H11; assumption.
-
-apply t_letdia_get_LF with (L:=L) (A:=A) (G:=G) (Gamma:=Gamma_subst).
-rewrite subst_t__inner.
-eapply IHHT with (Gamma_TS := Gamma_subst) (Gamma_HT0 := Gamma_subst & A0) (w1 := w) (A1:=A0); eauto.
-
-apply ok_Bg_permut with (G:=(w0, Gamma_HT) :: G0).
-apply permut_trans with (l2:=((w0, Gamma_HT)::(w, Gamma_subst & A0) :: G)).
-permut_simpl.
-apply permut_trans with (l2:= (G1 & (w, Gamma_subst & A0))).
-assumption.
-permut_simpl. apply permut_sym; assumption.
-permut_simpl.
-assumption.
-
-apply BackgroundSubsetImpl with (G:=emptyEquiv G_min); eauto.
-exists (@nil Context_LF). 
-apply permut_trans with (l2:=emptyEquiv (G1 & (w0, Gamma_HT))).
-apply emptyEquiv_permut in H2; rew_app; assumption.
-apply emptyEquiv_permut; apply permut_sym; apply permut_app_l; assumption.
-
-intros.
-rewrite subst_t__outer with (w':=fctx w0).
-unfold open_ctx;
-rewrite <- subst_order_irrelevant; eauto.
-eapply H with (G0:=(w',A::nil)::G1) (A1:=A0); eauto.
-
-skip. (* ok_Bg *)
-permut_simpl; assumption.
-permut_simpl; assumption.
-skip. (* ok_Bg *) 
-skip. (* ok_Bg *)
-
-apply BackgroundSubsetImpl with (G:= (nil & (w', nil) ++ emptyEquiv G_min)).
-apply GlobalWeakening. rew_app. assumption.
-exists (@nil Context_LF); permut_simpl. simpl. permut_simpl. 
-apply emptyEquiv_permut. assumption.
-assumption.
-apply permut_trans with (l2:=G1 & (w, Gamma_subst)).
-permut_simpl; assumption.
-apply permut_sym; assumption.
-
-(* stay in outer *)
-assert (exists GH, exists GT, G1 = GH & (w, Gamma) ++ GT).
-apply permut_split_neq with (G:=G) (G':=nil) (elem':=(w_subst, Gamma_subst & A0)).
-intro nn; inversion nn; subst; elim H10; reflexivity.
-apply permut_trans with (l2:=G0). 
-rew_app; assumption.
-assumption.
-
-destruct H11 as [GH]; destruct H11 as [GT].
-apply t_letdia_get_LF with (G:=GH++GT & (w_subst, Gamma_subst)) (Gamma:=Gamma) (L:=L)(A:=A).
-rewrite subst_t__outer with (w':= fctx w).
-subst.
-eapply IHHT with (Gamma_subst := Gamma_subst) (w_subst:=w_subst) (w1:=w) (G0:=GH ++ GT & (w0, Gamma_HT)) (G_TS:=(GH++GT & (w_subst, Gamma_subst)) & (w0, Gamma_HT)) (A0:=A0); eauto.
-
-apply ok_Bg_permut with (G:=(w0, Gamma_HT) :: G0).
-apply permut_trans with (l2:= (w0, Gamma_HT) :: (G & (w, Gamma))).
-permut_simpl. apply permut_sym; assumption.
-permut_simpl.
-assumption.
-
-apply permut_trans with (l2:=((GH ++ GT & (w_subst, Gamma_subst & A0)) & (w0, Gamma_HT))).
-apply permut_app_l.
-assert (permut (G & (w, Gamma)) ((GH & (w, Gamma) ++ GT) & (w_subst, Gamma_subst & A0))). 
-apply permut_trans with (l2:=G0); assumption.
-replace G with (G++nil).
-replace (GH ++ GT & (w_subst, Gamma_subst & A0)) with (GH ++ GT & (w_subst, Gamma_subst & A0) ++ nil).
-apply permut_inv with (elem:=(w, Gamma)).
-rew_app in *; assumption.
-rew_app; reflexivity.
-rew_app; reflexivity.
-permut_simpl.
-
-permut_simpl.
-intro nn; subst; elim H10; reflexivity.
-
-apply ok_Bg_permut with (G:= (w_subst, nil):: G_min).
-permut_simpl.
-apply permut_trans with (l2:=(GH & (w, Gamma) ++ GT) & (w0, Gamma_HT)).
-assumption.
-permut_simpl.
-assumption.
-
-skip. (* ok_Bg *)
-
-apply BackgroundSubsetImpl with (G:=emptyEquiv G_min).
-eassumption.
-exists (@nil Context_LF).
-apply permut_trans with (l2:=emptyEquiv ((GH & (w, Gamma) ++ GT) & (w0, Gamma_HT))).
-apply emptyEquiv_permut in H2; rew_app in *; assumption.
-apply emptyEquiv_permut; permut_simpl.
-assumption.
-
-intros.
-rewrite subst_t__outer with (w':=fctx w0).
-unfold open_ctx;
-rewrite <- subst_order_irrelevant; eauto.
-eapply H with (G0:=(w',A::nil)::G1) (A0:=A0); eauto.
-
-skip. (* ok_Bg *)
-
-permut_simpl.
-apply permut_trans with (l2:=G0); assumption.
-
-rewrite H11; 
-permut_simpl.
-
-skip. (* ok_Bg *)
-skip. (* ok_Bg *)
-
-apply BackgroundSubsetImpl with (G:=nil & (w', nil) ++ emptyEquiv G_min).
-apply GlobalWeakening.
-rew_app. assumption.
-exists (@nil Context_LF).
-permut_simpl; simpl. permut_simpl.
-apply emptyEquiv_permut. assumption.
-assumption.
-
-apply permut_trans with (l2:=G1 & (w_subst, Gamma_subst)). 
-subst; permut_simpl.
-apply permut_sym; assumption.
-Admitted. (* Existential variable non-instantiated *)
-
-Lemma subst_t_preserv_types_end_inner:
-forall Gamma G M N A B w
-  (Ok: ok_Bg ((w, Gamma & A)::G) nil)
-  (HM: emptyEquiv G |= (w, nil) |- M ::: A)
-  (HT: G |= (w, Gamma & A) |- N ::: B)
-  (H_lc: lc_w_LF M),
-  G |= (w, Gamma) |- [ M // length Gamma | fctx w] [N | fctx w] ::: B.
-intros;
-eapply subst_t_preserv_types_end with (Gamma_HT := Gamma & A); eauto. 
-Qed.
-
-Lemma subst_t_preserv_types_end_outer:
-forall G0 w w_subst Gamma_subst A G' G_HT G_TS Gamma M N B
-  (Ok_G': ok_Bg ((w_subst, nil)::G') nil)
-  (Ok_GHT: ok_Bg ((w,Gamma)::G_HT) nil)
-  (H_G': permut G' (G0 & (w, Gamma)))
-  (H_G'': permut G_HT (G0 & (w_subst, Gamma_subst & A)))
-  (H_G''': permut G_TS (G0 & (w_subst, Gamma_subst)))
-  (HM: emptyEquiv G' |= (w_subst, nil) |- M ::: A)
-  (H_lc: lc_w_LF M)
-  (HT: G_HT |= (w, Gamma) |- N ::: B),
-  G_TS |= (w, Gamma) |- [ M // length Gamma_subst | fctx w_subst ] [N | fctx w] ::: B.
-intros;
-eapply subst_t_preserv_types_end; eauto.
-intro; absurd (w_subst = w); auto.
-apply emptyEquiv_permut in H_G';
-eapply unique_worlds with (G:=emptyEquiv G0); eauto;
-eapply BackgroundSubsetImpl with (G:=emptyEquiv G'); eauto.
-exists (@nil Context_LF); rew_app.
-rewrite emptyEquiv_last with (G':=emptyEquiv G0) in H_G'.
-eassumption.
-auto.
-rewrite ok_Bg_emptyEquiv.
-apply ok_Bg_permut with (G:=emptyEquiv ((w, Gamma)::G_HT)).
-simpl; permut_simpl.
-apply permut_trans with (l2:=emptyEquiv(G0 & (w_subst, Gamma_subst & A))).
-apply emptyEquiv_permut in H_G''; assumption.
-apply permut_trans with (l2:=emptyEquiv(G0 & (w_subst, Gamma_subst))).
-rewrite emptyEquiv_last with (G':=emptyEquiv G0).
-rewrite emptyEquiv_last with (G':=emptyEquiv G0).
-permut_simpl.
-reflexivity. reflexivity.
-apply emptyEquiv_permut in H_G'''. apply permut_sym; assumption.
-rewrite ok_Bg_emptyEquiv in Ok_GHT. simpl in Ok_GHT.
-simpl. assumption.
-Qed.
-
-Lemma subst_t_preserv_types:
-forall L Delta G0 G_min G_HT G_TS Gamma_HT Gamma_TS w_subst Gamma_subst w N A
-  (H_L: subst_typing G_min L Delta w_subst)
-  (H_lc: forall M, Mem M L -> lc_w_LF M)
-  (H_inner: w_subst = w -> G_HT = G_min /\ G_HT = G_TS /\ Gamma_HT = Gamma_TS ++ Delta /\
-            permut G0 G_HT /\ Gamma_subst = Gamma_TS)
-  (H_outer: w_subst <> w -> Gamma_HT = Gamma_TS /\ permut G_min (G0 & (w, Gamma_HT)) /\
-            permut G_HT (G0 & (w_subst, Gamma_subst ++ Delta)) /\ 
-            permut G_TS (G0 & (w_subst, Gamma_subst)))
-  (HOk: ok_Bg ((w, Gamma_HT) :: G_HT) nil)
-  (HT: G_HT |= (w, Gamma_HT) |- N ::: A),
-  G_TS |= (w, Gamma_TS) |- subst_list L (length Gamma_subst) N (fctx w_subst) (fctx w) ::: A.
-induction L; destruct Delta; simpl in *; intros; try contradiction;
-unfold subst_t;
-destruct (eq_var_LF_dec w_subst w).
-(* = - inner substitution, nil *)
-apply H_inner in e; destruct e; destruct H0; destruct H1; destruct H2.
-subst G_TS; subst Gamma_HT.
-replace Gamma_TS with (Gamma_TS ++ nil) by (rew_app; reflexivity).
-  assumption.
-(* <> - outer substitution, nil *)
-apply H_outer in n; destruct n; destruct H0; destruct H1.
-rew_app in H1; apply BackgroundSubsetImpl with (G:=G_HT).
-subst Gamma_TS; assumption.
-exists (@nil Context_LF); permut_simpl;
-apply permut_trans with (l2:=(G0 & (w_subst, Gamma_subst))).
-  assumption.
-  apply permut_sym; assumption.
-(* = - inner substitution, step *)
-case_if; try (inversion H; discriminate); clear H.
-assert (w_subst = w) by assumption.
-apply H_inner in H; destruct H; destruct H0; destruct H1; destruct H2;
-clear H_inner H_outer;
-destruct H_L;
-rewrite subst_t__inner.
-subst Gamma_subst. subst w_subst;
-apply subst_t_preserv_types_end_inner with (A:=t);
-subst G_min; subst G_TS;
-case_if. simpl. case_if. assumption.
-assumption.
-replace (S(length Gamma_TS)) with (length (Gamma_TS & t) ).
-eapply IHL; eauto. 
-intros; apply H_lc; apply Mem_next; assumption.
-intro n; elim n. reflexivity.
-case_if; assumption.
-subst Gamma_HT; rew_app in *; assumption.
-rew_length; omega.
-apply H_lc; apply Mem_here.
-(* <> - outer substitution, step *)
-case_if; clear H.
-assert (w_subst <> w) by assumption.
-apply H_outer in H. destruct H. destruct H0; destruct H1.
-clear H_inner H_outer.
-destruct H_L.
-rewrite subst_t__outer with (w':=fctx w).
-subst.
-eapply subst_t_preserv_types_end_outer with (A:=t) (G_HT := (G0&(w_subst, Gamma_subst & t))); eauto.
-apply ok_Bg_permut with (G:=(w, Gamma_TS) :: G0 & (w_subst, nil)).
-permut_simpl.
-apply permut_trans with (l2:=G0 & (w, Gamma_TS)).
-permut_simpl; apply permut_sym; assumption.
-apply permut_sym; assumption.
-simpl.
-case_if.
-apply ok_Bg_permut with (G':=G0 & (w_subst, Gamma_subst ++ t::Delta)) in HOk. 
-rewrite ok_Bg_emptyEquiv in HOk.
-rewrite emptyEquiv_last with (G':=emptyEquiv G0) in HOk.
-rewrite ok_Bg_emptyEquiv.
-rewrite emptyEquiv_last with (G':=emptyEquiv G0).
-assumption.
-reflexivity.
-reflexivity. 
-assumption.
-simpl; case_if.
-rewrite ok_Bg_emptyEquiv in HOk.
-apply ok_Bg_permut with (G':=emptyEquiv(G0 & (w_subst, Gamma_subst & t))) in HOk.
-rewrite ok_Bg_emptyEquiv;
-assumption.
-apply permut_trans with (l2:=emptyEquiv (G0 & (w_subst, Gamma_subst ++ t :: Delta))).
-apply emptyEquiv_permut; assumption.
-rewrite emptyEquiv_last with (G':=emptyEquiv G0).
-apply permut_sym;
-rewrite emptyEquiv_last with (G':=emptyEquiv G0).
-permut_simpl. reflexivity.
-reflexivity.
-apply H_lc; apply Mem_here.
-replace (S(length Gamma_subst)) with (length (Gamma_subst & t) ).
-eapply IHL; eauto.
-intros; apply H_lc; apply Mem_next; assumption.
-intro nn; elim n; subst w; reflexivity.
-case_if. apply ok_Bg_permut with (G:=G_HT); rew_app in *; assumption.
-apply BackgroundSubsetImpl with (G:=G_HT).
-assumption.
-exists (@nil Context_LF); permut_simpl; rew_app in *; assumption.
-rew_length; omega.
-intro nn; inversion nn; subst; elim n; reflexivity.
-Qed.
-
-Lemma subst_t_preserv_types_inner:
-forall L G Gamma w Delta N B
-  (HT_L: subst_typing G L Delta w)
-  (HT_lc: forall M, Mem M L -> lc_w_LF M)
-  (HOk: ok_Bg ((w, Gamma++Delta)::G) nil)
-  (HT_N: G |= (w, Gamma ++ Delta) |- N ::: B),
-  G |= (w, Gamma) |- subst_list L (length Gamma) N (fctx w) (fctx w) ::: B.
-intros;
-eapply subst_t_preserv_types; eauto.
-intro n; elim n; reflexivity.
-Qed.
-
-Lemma subst_t_preserv_types_outer:
-forall L G0 G G' G'' Gamma Gamma' w w' Delta N B
-  (HT_G0: permut G (G0 & (w', Gamma')))
-  (HT_G': permut G' (G0 & (w, Gamma))) 
-  (HT_G'': permut G'' (G0 & (w', Gamma' ++ Delta)))
-  (HT_L: subst_typing G' L Delta w')
-  (HT_lc: forall M, Mem M L -> lc_w_LF M)
-  (HOk: ok_Bg ((w, Gamma)::G'') nil)
-  (HT_N: G'' |= (w, Gamma) |- N ::: B),
-  G |= (w, Gamma) |- subst_list L (length Gamma') N (fctx w') (fctx w)  ::: B.
-intros;
-eapply subst_t_preserv_types; eauto.
-intro n; absurd (w = w'); try symmetry; auto.
-eapply unique_worlds; eauto.
-Qed.
-
-Lemma inv_subst_ctx_preserv_types:
-forall G_HT G_TS G0 Gamma_HT Gamma_TS Gamma_fresh Gamma_subst w_TS w_HT 
-       w_fresh w_subst w_step M A k
-  (Fresh: w_fresh \notin free_worlds_LF M)
-  (H_outer: w_subst <> w_TS -> w_fresh <> w_TS ->
-            w_TS = w_HT /\ G_HT = G_TS /\ Gamma_HT = Gamma_TS /\
-            permut G_HT (G0 & (w_subst, Gamma_fresh ++ Gamma_subst)))
-  (H_old: w_subst = w_HT -> w_step = w_fresh -> 
-            w_TS = w_HT /\ G_HT = G_TS /\ Gamma_TS = Gamma_HT /\
-            G0 = G_HT /\ Gamma_HT = Gamma_fresh ++ Gamma_subst)
-  (H_new: w_subst = w_fresh -> w_subst = w_HT ->
-            w_TS = w_HT /\ w_HT = w_step /\
-            w_TS = w_HT /\ w_HT = w_step /\
-            Gamma_TS = Gamma_HT /\ Gamma_HT = Gamma_fresh ++ Gamma_subst)
-  (HT: G_HT |= (w_HT, Gamma_HT) |- {{ fctx w_subst // fctx w_fresh }} 
-                                   [ {{fctx w_fresh // bctx k }}  [ M | fctx w_step, 0, 0] |
-                                     fctx w_step, length Gamma_fresh, 0] ::: A),
-  G_TS |= (w_TS, Gamma_TS) |- {{ fctx w_subst // bctx k }} [ M | fctx w_TS, 0, 0] ::: A.
-Admitted.
-
-Lemma inv_subst_ctx_preserv_types_outer:
-forall G0 G w w' w0 Gamma Gamma' Gamma0 M A k
-  (Fresh: w' \notin free_worlds_LF M)
-  (HT_G: permut G (G0 & (w, Gamma' ++ Gamma)))
-  (HT: G |= (w0, Gamma0) |- {{ fctx w // fctx w'}} 
-    [ {{fctx w' // bctx k}} [M | fctx w0, 0, 0] | fctx w0, (length Gamma'), 0] ::: A),
-  G |= (w0, Gamma0) |- {{fctx w // bctx k}}[M | fctx w0, 0, 0] ::: A.
-intros;
-assert (w0 <> w) by (eapply unique_worlds; eauto);
-eapply inv_subst_ctx_preserv_types 
-  with (w_TS:=w0) (w_subst:=w) (w_fresh:=w') (w_step:=w0) (
-G0:=G0);
-eauto.
-intro n; symmetry in n; contradiction.
-intros m n; symmetry in n; contradiction.
-Qed.
-
-Lemma inv_subst_ctx_preserv_types_new:
-forall G w w' Gamma Gamma' M A k
-  (Fresh: w' \notin free_worlds_LF M)
-  (HT: G |= (w, Gamma' ++ Gamma) |- {{fctx w // fctx w'}} 
-    [ {{ fctx w' // bctx k }} [M | fctx w, 0,0] | fctx w, length Gamma',0] ::: A),
-  G |= (w, Gamma'++Gamma) |- {{fctx w // bctx k }}[ M | fctx w, 0,0] ::: A.
-intros; 
-eapply inv_subst_ctx_preserv_types with (w_HT:=w);
-eauto.
-intro n; elim n; reflexivity.
-intros; repeat split; auto.
-Qed.
-
-Lemma inv_subst_ctx_preserv_types_old:
-forall G w w' Gamma Gamma' M A k
-  (Fresh: w' \notin free_worlds_LF M)
-  (HT: G |= (w, Gamma'++Gamma) |- {{fctx w // fctx w'}} 
-    [ {{ fctx w' // bctx k }} [M | fctx w', 0,0] | fctx w', length Gamma',0] ::: A),
-  G |= (w, Gamma'++Gamma) |- {{fctx w // bctx k }}[ M | fctx w, 0,0] ::: A.
-intros; 
-eapply inv_subst_ctx_preserv_types with (w_step:=w');
-eauto.
-intro n; elim n; reflexivity.
-intros; repeat split; auto.
-Qed.
-
-Lemma rename_ctx_preserv_types:
-forall G w Gamma M A k
-  (Ok: ok_Bg ((w, Gamma)::G) nil)
-  (HT: G |= (w, Gamma) |- M ::: A),
-  forall G0 G' w0 w1 Gamma0 Gamma1,
-  ( permut G (G0 & (w0, Gamma0) & (w1, Gamma1)) ->
-    permut G' (G0 & (w0, Gamma1 ++ Gamma0)) ->
-    G' |= (w, Gamma) |- {{fctx w0 // fctx w1}} [M | fctx w, length Gamma1, k] ::: A)
-  /\
-  ( permut G (G0 & (w0, Gamma0)) ->
-    permut G' G0 ->
-    G' |= (w0, Gamma ++ Gamma0) |- {{fctx w0 // fctx w}} [ M | fctx w, length Gamma, k] ::: A)
-  /\
-  ( permut G (G0 & (w1, Gamma1)) ->
-    permut G' G0 ->
-    G' |= (w, Gamma1 ++ Gamma) |- {{fctx w // fctx w1}} [M | fctx w, length Gamma1, k] ::: A)
-.
-Admitted.
-
-Lemma rename_ctx_preserv_types_outer:
-forall G G' G'' w w' w0 Gamma Gamma' Gamma0 M A
-  (Ok: ok_Bg ((w0, Gamma0)::G') nil)
-  (HT_G': permut G' (G & (w, Gamma) & (w', Gamma')))
-  (HT_G'': permut G'' (G & (w, Gamma' ++ Gamma)))
-  (HT: G' |= (w0, Gamma0) |- M ::: A),
-  G'' |= (w0, Gamma0) |- {{fctx w // fctx w'}} [M | fctx w0, length (Gamma'), 0] ::: A.
-intros;
-eapply rename_ctx_preserv_types; eauto.
-Qed.
-
-Lemma rename_ctx_preserv_types_old:
-forall G G' w0 w1 Gamma0 Gamma1 M A
-  (Ok: ok_Bg ((w1, Gamma0)::G') nil)
-  (HT_G': permut G' (G & (w0, Gamma0)))
-  (HT: G' |= (w1, Gamma1) |- M ::: A),
-  G |= (w0, Gamma1++Gamma0) |- {{fctx w0 // fctx w1}} [M | fctx w1, length (Gamma1), 0] ::: A.
-intros;
-eapply rename_ctx_preserv_types; eauto.
-Qed.
-
-Lemma rename_ctx_preserv_types_new:
-forall G G' w0 w1 Gamma0 Gamma1 M A
-  (Ok: ok_Bg ((w0,Gamma0)::G') nil)
-  (HT_G': permut G' (G & (w1, Gamma1)))
-  (HT: G' |= (w0, Gamma0) |- M ::: A),
-  G |= (w0, Gamma1++Gamma0) |- {{fctx w0 // fctx w1}} [M | fctx w0, length (Gamma1), 0] ::: A.
-intros;
-eapply rename_ctx_preserv_types; eauto.
-Qed.
-
-Lemma Progress:
-forall G w M A
-  (H_lc: lc_w_LF M)
-  (HT: emptyEquiv G |= (w, nil) |- M ::: A),
-  value_LF M \/ exists N, (M, fctx w) |-> (N, fctx w).
-intros.
-remember (w, (@nil ty_LF)) as Ctx.
-generalize dependent Ctx.
-generalize dependent A.
-generalize dependent w.
-generalize dependent G. 
-induction M; intros; eauto using value_LF;
-inversion HeqCtx; subst.
-(* hyp *)
-inversion HT; destruct n;
-apply Nth_nil_inv in HT0; contradiction.
-(* appl *)
-right; inversion HT; subst.
-inversion H_lc; subst.
-destruct IHM1 with (Ctx := (w, (@nil ty_LF))) (G := G) (A := A0 ---> A) (w := w);
-auto.
-  inversion H0; subst; inversion HT1; subst; eexists; constructor.
-  inversion H2; subst; assumption.
-  assumption.
-  destruct H0; eexists; constructor. 
-  eapply H0.
-  assumption.
-  assumption.
-(* unbox & unbox_fetch *)
-right; inversion HT; subst.
-(* unbox *)
-inversion H_lc; subst.
-destruct IHM with (Ctx := (w, (@nil ty_LF))) (G := G) (A := [*]A) (w := w);
-auto.
-  inversion H0; subst; inversion HT0; subst; eexists; constructor. 
-  inversion H3; subst; assumption.
-  destruct H0; eexists; constructor.
-  eapply H0.
-  apply closed_w_succ; assumption.
-(* unbox_fetch *)
-assert (Gamma = nil).
-  apply emptyEquiv_nil with (G:=G) (G':=G0 & (w0, Gamma)) (w:=w0).
-  apply permut_sym; assumption.
-  rewrite Mem_app_or_eq; right; rewrite Mem_cons_eq; left; reflexivity.
-subst. 
-inversion H_lc; subst;
-destruct IHM with (Ctx := (w0, (@nil ty_LF))) (G := G0 & (w, nil)) (A:=[*]A) (w:=w0).
-assumption.
-reflexivity.
-assert (emptyEquiv (G0 & (w, nil)) = G0 & (w, nil)).
-apply emptyEquiv_last.
-apply emptyEquiv_inv with (w:=w0).
-apply emptyEquiv_empty with (G := G).
-  apply permut_sym; assumption.
-rewrite H0; assumption.
-inversion H0; subst; inversion HT0; subst. 
-eexists; constructor.
-inversion H3; subst; assumption.
-destruct H0 as [M'].
-eexists; constructor. eassumption. apply closed_w_succ; assumption.
-(* here & get_here *)
-inversion HT; subst.
-(* here *)
-inversion H_lc; subst.
-destruct IHM with (G:=G) (w:=w) (A:=A0) (Ctx:=(w, (@nil ty_LF))); auto.
-left; apply val_get_here_LF; assumption.
-right; destruct H0; exists (get_here_LF (fctx w) x); eauto using step_LF.
-(* get_here *)
-inversion H_lc; subst;
-assert (Gamma = nil).
-  apply emptyEquiv_nil with (G:=G) (G':=G0 & (w0, Gamma)) (w:=w0).
-  apply permut_sym; assumption.
-  rewrite Mem_app_or_eq; right; rewrite Mem_cons_eq; left; reflexivity.
-subst; destruct (IHM H3 (G0 & (w, nil)) w0 A0 (w0,nil)); auto.
-assert (emptyEquiv (G0 & (w, nil)) = G0 & (w, nil)).
-apply emptyEquiv_last.
-apply emptyEquiv_inv with (w:=w0).
-apply emptyEquiv_empty with (G := G).
-  apply permut_sym; assumption.
-rewrite H0; assumption.
-left; econstructor; eassumption.
-right; destruct H0; eexists; constructor; eassumption. 
-(* letdia & letdia_get *)
-inversion HT; subst;
-inversion H_lc; subst.
-(* letdia *)
-right;
-destruct IHM1 with  (G:=G) (w:=w) (A:=<*>A0) (Ctx:=(w, (@nil ty_LF))); auto.
-inversion H0; subst; inversion HT1; subst.
-  eexists; econstructor. 
-  inversion H5; subst; assumption.
-  eassumption.
-  eexists; econstructor. inversion H5; subst; assumption. eassumption.
-destruct H0; exists (letdia_get_LF (fctx w) x M2); eauto using step_LF.
-(* letdia_get *)
-right;
-assert (Gamma = nil).
-  apply emptyEquiv_nil with (G:=G) (G':=G0 & (w0, Gamma)) (w:=w0).
-  apply permut_sym; assumption.
-  rewrite Mem_app_or_eq; right; rewrite Mem_cons_eq; left; reflexivity.
-subst; destruct (IHM1 H5 (G0 & (w, nil)) w0 (<*>A0) (w0,nil)); auto.
-assert (emptyEquiv (G0 & (w, nil)) = G0 & (w, nil)).
-apply emptyEquiv_last.
-apply emptyEquiv_inv with (w:=w0).
-apply emptyEquiv_empty with (G := G).
-  apply permut_sym; assumption.
-rewrite H0; assumption.
-inversion H0; subst; inversion HT1; subst.
-  eexists; econstructor; eauto.
-  inversion H5; subst; assumption.
-  eexists; econstructor; eauto.
-  inversion H5; subst; eassumption.
-  destruct H0; eexists; econstructor; eassumption.
-Qed.
 
 Lemma Fresh: 
   forall (L:fset var), exists w0, w0 \notin L.
@@ -1917,15 +144,736 @@ exists (var_gen L);
 apply var_gen_spec.
 Qed.
 
+Lemma GlobalWeakening:
+forall G G' Ctx Ctx' M A
+  (HT: G ++ G' |= Ctx |- M ::: A),
+  G & Ctx' ++ G' |= Ctx |- M ::: A.
+Admitted.
+
+Lemma WeakeningBackgroundElem:
+forall G G' w Delta Delta' Ctx M A
+  (HT: G & (w, Delta) ++ G' |= Ctx |- M ::: A),
+  G & (w, Delta ++ Delta') ++ G' |= Ctx |- M ::: A.
+Admitted.
+
+Lemma Weakening:
+forall G w Gamma Gamma' M A
+  (HT: G |= (w, Gamma) |- M ::: A),
+  G |= (w, Gamma ++ Gamma') |- M ::: A.
+Admitted.
+
+(* emptyEquiv = map (fun x => (x, nil)) (map fst G) *)
+Fixpoint emptyEquiv (G: Background_LF) : Background_LF :=
+match G with
+| nil => nil
+| (w, a)::G => (w, nil) :: emptyEquiv G
+end.
+
+Lemma subst_t_preserv_types:
+forall L G w Gamma A B M N v
+  (H_lc_t: lc_t_LF M)
+  (H_lc_w: lc_w_LF M)
+  (Fresh: v \notin L) 
+  (HT: G |= (w, Gamma) |- N ::: B), 
+  ( forall Gamma0,
+    Gamma = (v, A) :: Gamma0 ->
+    emptyEquiv G |= (w, nil) |- M ::: A ->
+  (* "inner" substitution *)
+    G |= (w, Gamma0) |- N ^t^ M ::: B) /\
+  (* "outer" substitution *)
+  ( forall G0 G' G'' w' Gamma',
+    permut G (G0 & (w', (v,A)::Gamma')) ->
+    permut G' (G0 & (w, Gamma)) ->
+    permut G'' (G0 & (w', Gamma')) ->
+    emptyEquiv G' |= (w', nil) |- M ::: A ->
+    G'' |= (w, Gamma) |- N ^t^ M ::: B).
+Admitted.
+
+Lemma subst_t_preserv_types_inner:
+forall L G w Gamma A B M N
+  (H_lc_t: lc_t_LF M)
+  (H_lc_w: lc_w_LF M)
+  (HT: forall v, v \notin L -> 
+    G |= (w, (v, A) :: Gamma) |- N ::: B)
+  (HM: emptyEquiv G |= (w, nil) |- M ::: A),
+  G |= (w, Gamma) |- N ^t^ M ::: B.
+intros;
+assert (exists v, v \notin L) as HF by apply Fresh;
+destruct HF as (v_fresh);
+eapply subst_t_preserv_types with (Gamma := (v_fresh, A) :: Gamma); eauto.
+Qed.  
+
+Lemma subst_t_preserv_types_outer:
+forall L G0 G' G'' w w' Gamma Gamma' A B M N
+  (H_lc_t: lc_t_LF M)
+  (H_lc_w: lc_w_LF M)
+  (G0G': permut G' (G0 & (w, Gamma)))
+  (HM: emptyEquiv G' |= (w', nil) |- M ::: A)
+  (HT: forall G v, v \notin L -> 
+    permut G (G0 & (w', (v, A) :: Gamma')) ->
+    G |= (w, Gamma) |- N ::: B)
+  (G0G'': permut G'' (G0 & (w', Gamma'))),
+  G'' |= (w, Gamma) |- N ^t^ M ::: B.
+intros; 
+assert (exists v, v \notin L) as HF by apply Fresh;
+destruct HF as (v_fresh);
+eapply subst_t_preserv_types with (Gamma := Gamma); eauto.
+Qed.  
+
+Lemma rename_w_preserv_types:
+forall G w Gamma A M G' w' Gamma'
+  (HT: G |= (w, Gamma) |- M ::: A),
+  (* "new" substitution *)
+  ( permut G (G' & (w', Gamma')) ->
+    G' |= (w, Gamma ++ Gamma') |- {{ fctx w // fctx w' }} M ::: A) /\
+  (* "old" substitution *)
+  ( permut G (G' & (w', Gamma')) ->
+    G' |= (w', Gamma' ++ Gamma) |- {{ fctx w' // fctx w }} M ::: A) /\
+  (* "outer" substitution *)
+  (forall G0 w'' Gamma'',
+    permut G (G0 & (w', Gamma') & (w'', Gamma'')) ->
+    permut G' (G0 & (w', Gamma' ++ Gamma'')) ->
+    G' |= (w, Gamma) |- {{ fctx w' // fctx w''}} M ::: A).
+intros;
+remember (w, Gamma) as Ctx;
+generalize dependent Gamma;
+generalize dependent w;
+generalize dependent w';
+generalize dependent Gamma';
+generalize dependent G';
+induction HT; repeat split; intros;
+inversion HeqCtx; subst;
+simpl in *.
+(* hyp *)
+constructor;
+[ skip | (* ok_Bg will need some lemmas later on *)
+  rewrite Mem_app_or_eq; left; auto].
+constructor;
+[ skip | (* ok_Bg *)
+  rewrite Mem_app_or_eq; right; auto].
+constructor; 
+[ skip | (* ok_Bg *) 
+  auto].
+(* lam *)
+apply t_lam_LF with (L := L);
+[ skip | (* ok_Bg *)
+  intros]; unfold open_var in *;
+rewrite subst_order_irrelevant_free;
+try (eapply H with (v':=v') (G':=G') (Gamma := (v',A)::Gamma0));
+eauto;
+simpl; apply notin_empty. 
+apply t_lam_LF with (L := L);
+[ skip | (* ok_Bg *)
+  intros]; unfold open_var in *;
+rewrite subst_order_irrelevant_free;
+edestruct H; eauto; destruct H3; 
+replace ((v', A) :: Gamma' ++ Gamma0) with (Gamma' ++ (v', A) :: Gamma0)
+  by skip; (* TODO: order of elems in context is irrelevant *)
+eauto;
+apply notin_empty. 
+apply t_lam_LF with (L := L);
+[ skip | (* ok_Bg *)
+  intros]; unfold open_var in *;
+rewrite subst_order_irrelevant_free;
+edestruct H; eauto; destruct H4;
+eauto;
+simpl; apply notin_empty. 
+(* appl *)
+apply t_appl_LF with (A:=A);
+[ skip |  (* ok_Bg *)
+  apply IHHT1 with (Gamma:=Gamma0) |
+  apply IHHT2 with (Gamma:=Gamma0) ]; 
+eauto.
+apply t_appl_LF with (A:=A);
+[ skip |  (* ok_Bg *)
+  apply IHHT1 with (Gamma:=Gamma0) |
+  apply IHHT2 with (Gamma:=Gamma0) ]; 
+eauto.
+apply t_appl_LF with (A:=A);
+[ skip |  (* ok_Bg *)
+  eapply IHHT1 |
+  eapply IHHT2 ]; 
+eauto.
+(* box *)
+apply t_box_LF with (L:=\{w'} \u L);
+[ skip | (* ok_Bg *)
+  intros]; 
+unfold open_ctx in *;
+rewrite notin_union in H1; destruct H1;
+rewrite notin_singleton in *;
+rewrite <- subst_ctx_comm; auto;
+eapply H; eauto;
+permut_simpl; assumption.
+apply t_box_LF with (L:=\{w0} \u L);
+[ skip | (* ok_Bg *)
+  intros]; 
+unfold open_ctx in *;
+rewrite notin_union in H1; destruct H1;
+rewrite notin_singleton in *;
+rewrite <- subst_ctx_comm; auto;
+eapply H; eauto;
+permut_simpl; assumption.
+apply t_box_LF with (L:=\{w''} \u L);
+[ skip | (* ok_Bg *)
+  intros]; 
+unfold open_ctx in *;
+rewrite notin_union in H2; destruct H2;
+rewrite notin_singleton in *;
+rewrite <- subst_ctx_comm; auto;
+eapply H with (G0:=G0 & (w0, Gamma0)) (Gamma':=Gamma') (Gamma'':=Gamma''); eauto;
+permut_simpl; rew_app in *; assumption.
+(* unbox *)
+case_if; 
+(* w0 = w' 
+   G ~=~ G' & (w', ..)
+   ok_Bg (w0, ..) G --> ok_Bg (w0,.. ) (G' & w' ,..)
+   -->
+   contradiction *)
+[ skip |
+  constructor];
+[ skip | (* ok_Bg *)
+  apply IHHT with (Gamma:=Gamma0); eauto].
+ 
+case_if; constructor;
+[ skip | (* ok_Bg *)
+  apply IHHT with (Gamma:=Gamma0); eauto].
+
+case_if; 
+(* ok_Bg ((w'', Gamma0) :: G) & G ~=~ (G0 & (w', ..) & (w'', ..)) -> contradiction*)
+[ skip | 
+  constructor];
+[ skip | (* ok_Bg *)
+  eapply IHHT; eauto].
+(* unbox_fetch *)
+case_if.
+(* G' ~=~ G & (w, Gamma)
+   G' ~=~ G'0 & (w'0, Gamma'0) -->
+   G'0 & (w'0, Gamma'0) ~= G & (w, Gamma) 
+   w = w'0
+   ok_Bg (w, Gamma) :: G -->
+   G'0 = G && Gamma'0 = Gamma *)
+assert (Gamma'0 = Gamma) by skip;
+assert (G'0 = G) by skip;
+inversion H1; subst;
+constructor;
+[ skip | (* ok_Bg *)
+  apply IHHT; auto].
+(* H: G & (w, Gamma) ~=~ G'
+   H0: G' ~=~ G'0 & (w'0, Gamma'0) -->
+   G'0 & (w'0, Gamma'0) ~= G & (w, Gamma) 
+   H1: w <> w'0 -->
+   exists GH, exists GT, G'0 = GH & (w, Gamma) ++ GT *)
+assert (exists GH, exists GT, G'0 = GH & (w, Gamma) ++ GT) as Split by skip;
+destruct Split as (GH, Split); destruct Split as (GT); subst.
+apply t_unbox_fetch_LF with (G:=GH++GT) (Gamma:=Gamma); 
+[ skip | (* ok_Bg *)
+  eapply IHHT; eauto | ]; 
+permut_simpl;
+(* H + H0 --> G & (w, Gamma) ~=~ GH & (w, Gamma) ++ GT & (w'0, Gamma'0) --> 
+   remove (w,Gamma) from both sides *)
+skip.
+
+case_if.
+(* w = w0 --> ok_Bg w,.. :: G & (w0, .. ) --> contradiction *)
+skip.
+destruct (eq_var_dec w w'0).
+(* w = w'0 follows that G = G'0 and Gamma = Gamma'0 *)
+assert (Gamma'0 = Gamma) by skip;
+assert (G'0 = G) by skip;
+subst; constructor; [skip | ].
+eapply IHHT with (w:=w'0) (Gamma1:=Gamma) (Gamma':=Gamma0); eauto.
+(* w <> w'0
+   H & H0 -> G'0 & (w'0, Gamma'0) ~=~ G & (w, Gamma) -->
+   exists GH, exists GT, G'0 = GH & (w, Gamma) ++ GT *)
+assert (exists GH, exists GT, G'0 = GH & (w, Gamma) ++ GT) as Split by skip;
+destruct Split as (GH, Split); destruct Split as (GT); subst.
+apply t_unbox_fetch_LF with (G:=GH++GT) (Gamma:=Gamma);
+[ skip | (* ok_Bg *)
+  eapply IHHT; eauto | ];
+permut_simpl.
+(* H + H0 --> G & (w, Gamma) ~=~ GH & (w, Gamma) ++ GT & (w'0, Gamma'0) --> 
+   remove (w,Gamma) from both sides *)
+skip.
+
+case_if.
+(* w = w'' 
+   (G0 & (w'0, Gamma'0) & (w'', Gamma'')) ~=~ G & (w, Gamma) -->
+   G0 & (w'0, Gamma'0) ~=~ G /\ Gamma'' = Gamma *)
+inversion H2;
+assert (permut G (G0 & (w'0, Gamma'0))) by skip;
+assert (Gamma'' = Gamma) by skip;
+subst.
+apply t_unbox_fetch_LF with (G:=G0) (Gamma:=Gamma'0 ++ Gamma).
+skip. (* ok_Bg *)
+apply IHHT; eauto.
+(* TODO: get rid of those 2 proofs, some permut_auto .. *)
+permut_simpl; assumption.
+apply permut_sym; assumption.
+assert (w <> w0) by skip. (* from ok_Bg *)
+destruct (eq_var_dec w w'0).
+(* w = w'0 follows that G = G'0 and Gamma = Gamma'0 *)
+assert (Gamma'0 = Gamma) by skip;
+assert (G'0 = G) by skip;
+subst. 
+(* ok_Bg w'0, Gamma :: G & (w0, Gamma0)
+   G ~=~ G0 & (w'0, Gamma ++ Gamma'') --->
+   variables from Gamma will be doubled; they should be unique;
+   contradiction *)
+skip.
+(* w <> w'0 /\ w <> w'
+   H & H0 -> G0 & (w'0, Gamma'0) & (w'', Gamma'') ~=~ G & (w, Gamma) -->
+   exists GH, exists GT, G0 = GH & (w, Gamma) ++ GT *)
+assert (exists GH, exists GT, G0 = GH & (w, Gamma) ++ GT) as Split by skip;
+destruct Split as (GH, Split); destruct Split as (GT); subst.
+apply t_unbox_fetch_LF with (G:=GH++GT & (w'0, Gamma'0++Gamma'')) (Gamma:=Gamma).
+skip.
+eapply IHHT with (w1:=w) (Gamma1:=Gamma) (G0:=GH++GT & (w0,Gamma0)) (Gamma':=Gamma'0) (Gamma'':=Gamma''); eauto.
+(* permut_auto desperately needed! *)
+permut_simpl; skip. (* H + H1 + permutation magic *)
+permut_simpl.
+apply permut_sym.
+apply permut_trans with (l2 := (GH & (w, Gamma) ++ GT) & (w'0, Gamma'0 ++ Gamma''));
+[auto | permut_simpl].
+(* here  -- same as unbox *)
+case_if; 
+(* w0 = w' 
+   G ~=~ G' & (w', ..)
+   ok_Bg (w0, ..) G --> ok_Bg (w0,.. ) (G' & w' ,..)
+   -->
+   contradiction *)
+[ skip |
+  constructor];
+[ skip | (* ok_Bg *)
+  apply IHHT with (Gamma:=Gamma0); eauto].
+ 
+case_if; constructor;
+[ skip | (* ok_Bg *)
+  apply IHHT with (Gamma:=Gamma0); eauto].
+
+case_if; 
+(* ok_Bg ((w'', Gamma0) :: G) & G ~=~ (G0 & (w', ..) & (w'', ..)) -> contradiction*)
+[ skip | 
+  constructor];
+[ skip | (* ok_Bg *)
+  eapply IHHT; eauto].
+
+(* get_here  -- same as unbox_fetch *)
+case_if.
+(* G' ~=~ G & (w, Gamma)
+   G' ~=~ G'0 & (w', Gamma') -->
+   G'0 & (w', Gamma') ~= G & (w, Gamma) 
+   w = w'
+   ok_Bg (w, Gamma) :: G -->
+   G'0 = G && Gamma' = Gamma *)
+assert (Gamma' = Gamma) by skip;
+assert (G'0 = G) by skip;
+inversion H2; subst;
+constructor;
+[ skip | (* ok_Bg *)
+  apply IHHT; auto].
+(* H: G & (w, Gamma) ~=~ G'
+   H0: G' ~=~ G'0 & (w', Gamma') -->
+   G'0 & (w', Gamma') ~= G & (w, Gamma) 
+   H1: w <> w' -->
+   exists GH, exists GT, G'0 = GH & (w, Gamma) ++ GT *)
+assert (exists GH, exists GT, G'0 = GH & (w, Gamma) ++ GT) as Split by skip;
+destruct Split as (GH, Split); destruct Split as (GT); subst.
+apply t_get_here_LF with (G:=GH++GT) (Gamma:=Gamma); 
+[ skip | (* ok_Bg *)
+  eapply IHHT; eauto | ]; 
+permut_simpl;
+(* H + H0 --> G & (w, Gamma) ~=~ GH & (w, Gamma) ++ GT & (w'0, Gamma'0) --> 
+   remove (w,Gamma) from both sides *)
+skip.
+
+case_if.
+(* w = w0 --> ok_Bg w,.. :: G & (w0, .. ) --> contradiction *)
+skip.
+destruct (eq_var_dec w w').
+(* w = w'0 follows that G = G'0 and Gamma = Gamma' *)
+assert (Gamma' = Gamma) by skip;
+assert (G'0 = G) by skip;
+subst; constructor; [skip | ].
+eapply IHHT with (w:=w') (Gamma1:=Gamma) (Gamma':=Gamma0); eauto.
+(* w <> w'0
+   H & H0 -> G'0 & (w'0, Gamma'0) ~=~ G & (w, Gamma) -->
+   exists GH, exists GT, G'0 = GH & (w, Gamma) ++ GT *)
+assert (exists GH, exists GT, G'0 = GH & (w, Gamma) ++ GT) as Split by skip;
+destruct Split as (GH, Split); destruct Split as (GT); subst.
+apply t_get_here_LF with (G:=GH++GT) (Gamma:=Gamma);
+[ skip | (* ok_Bg *)
+  eapply IHHT; eauto | ];
+permut_simpl.
+(* H + H0 --> G & (w, Gamma) ~=~ GH & (w, Gamma) ++ GT & (w'0, Gamma'0) --> 
+   remove (w,Gamma) from both sides *)
+skip.
+
+case_if.
+(* w = w'' 
+   (G0 & (w'0, Gamma'0) & (w'', Gamma'')) ~=~ G & (w, Gamma) -->
+   G0 & (w'0, Gamma'0) ~=~ G /\ Gamma'' = Gamma *)
+inversion H3;
+assert (permut G (G0 & (w', Gamma'))) by skip;
+assert (Gamma'' = Gamma) by skip;
+subst.
+apply t_get_here_LF with (G:=G0) (Gamma:=Gamma' ++ Gamma).
+skip. (* ok_Bg *)
+apply IHHT; eauto.
+(* TODO: get rid of those 2 proofs, some permut_auto .. *)
+permut_simpl; assumption.
+apply permut_sym; assumption.
+assert (w <> w0) by skip. (* from ok_Bg *)
+destruct (eq_var_dec w w').
+(* w = w'0 follows that G = G'0 and Gamma = Gamma'0 *)
+assert (Gamma' = Gamma) by skip;
+assert (G'0 = G) by skip;
+subst. 
+(* ok_Bg w'0, Gamma :: G & (w0, Gamma0)
+   G ~=~ G0 & (w'0, Gamma ++ Gamma'') --->
+   variables from Gamma will be doubled; they should be unique;
+   contradiction *)
+skip.
+(* w <> w'0 /\ w <> w'
+   H & H0 -> G0 & (w'0, Gamma'0) & (w'', Gamma'') ~=~ G & (w, Gamma) -->
+   exists GH, exists GT, G0 = GH & (w, Gamma) ++ GT *)
+assert (exists GH, exists GT, G0 = GH & (w, Gamma) ++ GT) as Split by skip;
+destruct Split as (GH, Split); destruct Split as (GT); subst.
+apply t_get_here_LF with (G:=GH++GT & (w', Gamma'++Gamma'')) (Gamma:=Gamma).
+skip.
+eapply IHHT with (w1:=w) (Gamma1:=Gamma) (G0:=GH++GT & (w0,Gamma0)) (Gamma':=Gamma') (Gamma'':=Gamma''); eauto.
+(* permut_auto desperately needed! *)
+permut_simpl; skip. (* H + H1 + permutation magic *)
+permut_simpl.
+apply permut_sym.
+apply permut_trans with (l2 := (GH & (w, Gamma) ++ GT) & (w', Gamma' ++ Gamma''));
+[auto | permut_simpl].
+(* letdia *)
+case_if.
+(* w0 = w' ->
+   ok_Bg w', Gamma0 :: G' & (w', Gamma') ->
+   contradiction *)
+skip.
+apply t_letdia_LF with (L_w:=L_w \u \{w'}) (L_t:=L_t) (A:=A).
+skip. (* ok_Bg *)
+eapply IHHT with (w:=w0) (Gamma:=Gamma0); eauto.
+intros. 
+rewrite notin_union in H3; destruct H3.
+rewrite notin_singleton in H4.
+unfold open_var in *; unfold open_ctx in *.
+rewrite <- subst_ctx_comm.
+rewrite subst_order_irrelevant_free.
+eapply H with (w:=w0) (Gamma:=Gamma0) (w':=w'0); eauto.
+permut_simpl; assumption.
+simpl; auto.
+intro; subst; elim H4; reflexivity.
+
+case_if.
+apply t_letdia_LF with (L_w:=L_w \u \{w0}) (L_t:=L_t) (A:=A).
+skip. (* ok_Bg *)
+eapply IHHT with (w:=w0) (Gamma:=Gamma0); eauto.
+intros. 
+rewrite notin_union in H3; destruct H3.
+rewrite notin_singleton in H4.
+unfold open_var in *; unfold open_ctx in *.
+rewrite <- subst_ctx_comm.
+rewrite subst_order_irrelevant_free.
+eapply H with (w:=w0) (Gamma:=Gamma0) (w':=w'0); eauto.
+permut_simpl; assumption.
+simpl; auto.
+intro; subst; elim H4; reflexivity.
+
+case_if.
+(* w0 = w'' -> H0 + Ok_Bg = contradiction *)
+skip. 
+apply t_letdia_LF with (L_w:=L_w \u \{w''}) (L_t:=L_t) (A:=A).
+skip. (* ok_Bg *)
+eapply IHHT with (w:=w0) (Gamma:=Gamma0); eauto.
+intros. 
+rewrite notin_union in H4; destruct H4.
+rewrite notin_singleton in H5.
+unfold open_var in *; unfold open_ctx in *.
+rewrite <- subst_ctx_comm.
+rewrite subst_order_irrelevant_free.
+eapply H with (w:=w0) (Gamma:=Gamma0) (G0:=G0 & ((w'0, (v', A)::nil))); eauto.
+permut_simpl; rew_app in *; eassumption.
+permut_simpl; assumption.
+simpl; auto.
+intro; subst; elim H5; reflexivity.
+(* letdia_get *)
+case_if.
+inversion H3; subst.
+(* w = w' ->
+   H1 + H0 = G & w', Gamma ~=~ G' & w', Gamma' ->
+   Gamma = Gamma' /\ G = G' *)
+assert (Gamma=Gamma') by skip;
+assert (G = G') by skip;
+subst.   
+eapply t_letdia_LF with (L_w := L_w \u \{w'}).
+skip. (* ok_Bg *)
+eapply IHHT; eauto.
+intros. 
+rewrite notin_union in H5; destruct H5.
+rewrite notin_singleton in H6.
+unfold open_var in *; unfold open_ctx in *.
+rewrite <- subst_ctx_comm.
+rewrite subst_order_irrelevant_free.
+eapply H with (w:=w0) (Gamma:=Gamma0); eauto.
+simpl; auto.
+intro; subst; elim H6; reflexivity.
+
+destruct (eq_var_dec w w0).
+subst; skip. (* ok_Bg -> contradiction *)
+(* H0 + H1: G & (w, Gamma) ~=~ G' & (w', Gamma') -->
+   exists GH, exists GT, G = GH & (w', Gamma') ++ GT *)
+assert (exists GH, exists GT, G' = GH & (w, Gamma) ++ GT) by skip;
+destruct H4 as (GH, H4); destruct H4 as (GT, H4).
+apply t_letdia_get_LF with (L_w:=L_w \u \{w'}) (L_t:=L_t) (A:=A) (G:=GH++GT) (Gamma:=Gamma).
+skip. (* ok_Bg *)
+eapply IHHT with (w1:=w) (G0:=GH++GT) (w':=w0) (Gamma':=Gamma0) (Gamma'':=Gamma');
+eauto.
+subst; permut_simpl. skip. (* H0 + H1 *)
+intros. 
+rewrite notin_union in H6; destruct H6.
+rewrite notin_singleton in H7.
+unfold open_var in *; unfold open_ctx in *.
+rewrite <- subst_ctx_comm.
+rewrite subst_order_irrelevant_free.
+eapply H with (w1:=w0) (Gamma1:=Gamma0); eauto.
+permut_simpl. skip. (* H0 + H1 *)
+simpl; auto.
+intro; subst; elim H7; auto.
+subst; permut_simpl.
+
+case_if.
+skip. (* w = w0 --> ok_Bg gives contradiction *)
+destruct (eq_var_dec w w').
+subst; skip. (* H0 + Ok_Bg gives contradiction *) 
+(* H0 + H1: G & (w, Gamma) ~=~ G' & (w', Gamma') -->
+   exists GH, exists GT, G = GH & (w', Gamma') ++ GT *)
+assert (exists GH, exists GT, G' = GH & (w, Gamma) ++ GT) by skip;
+destruct H4 as (GH, H4); destruct H4 as (GT, H4).
+apply t_letdia_get_LF with (L_w:=L_w \u \{w0}) (L_t:=L_t) (A:=A) (G:=GH++GT) (Gamma:=Gamma).
+skip. (* ok_Bg *)
+eapply IHHT; eauto.
+subst; permut_simpl. skip. (* H0 + H1 *)
+intros. 
+rewrite notin_union in H6; destruct H6.
+rewrite notin_singleton in H7.
+unfold open_var in *; unfold open_ctx in *.
+rewrite <- subst_ctx_comm.
+rewrite subst_order_irrelevant_free.
+eapply H with (w1:=w0) (Gamma1:=Gamma0); eauto.
+permut_simpl. skip. (* H0 + H1 + H4 *)
+simpl; auto.
+intro; subst; elim H7; auto.
+subst; permut_simpl.
+
+case_if.
+inversion H4; subst.
+(* H0 + H1 + Ok_Bg --> Gamma'' = Gamma & G0 & (w', Gamma') ~=~ G *)
+assert (Gamma'' = Gamma) by skip.
+assert (G1 & (w', Gamma') = G) by skip.
+subst.
+eapply t_letdia_get_LF with (G:=G1) (Gamma:=Gamma'++Gamma) (L_w:=L_w \u \{w''}).
+skip.
+eapply IHHT; eauto. 
+permut_simpl.
+intros. 
+unfold open_var in *; unfold open_ctx in *.
+rewrite <- subst_ctx_comm.
+rewrite subst_order_irrelevant_free.
+eapply H with (w:=w0) (G0:=(w'0, (v',A)::nil)::G1); eauto. 
+permut_simpl.
+permut_simpl.
+simpl; auto.
+rewrite notin_union in H6; 
+rewrite notin_singleton in H6;
+destruct H6; intro; elim H7; auto.
+apply permut_sym; auto.
+
+destruct (eq_var_dec w w').
+subst.
+(* H0 + H1 + Ok_Bg --> Gamma = Gamma' /\ G0 & (w'',Gamma'') = G *)
+assert (Gamma' = Gamma) by skip.
+assert (G1 & (w'', Gamma'') = G) by skip.
+subst.
+eapply t_letdia_get_LF with (G:=G1) (Gamma:=Gamma++Gamma'') (L_w:=L_w \u \{w''}).
+skip.
+eapply IHHT with (w:=w'); eauto. 
+permut_simpl.
+intros. 
+unfold open_var in *; unfold open_ctx in *.
+rewrite <- subst_ctx_comm.
+rewrite subst_order_irrelevant_free.
+eapply H with (w:=w0) (G0:=(w'0, (v',A)::nil)::G1) (Gamma':=Gamma); eauto. 
+permut_simpl.
+permut_simpl.
+simpl; auto.
+rewrite notin_union in H6; 
+rewrite notin_singleton in H6;
+destruct H6; intro; elim H7; auto.
+apply permut_sym; auto.
+(* H0 + H1: G & (w, Gamma) ~=~ G1 & (w', Gamma') & (w'', Gamma'') -->
+   exists GH, exists GT, G1 = GH & (w, Gamma) & (w', Gamma') ++ GT *)
+assert (exists GH, exists GT, G1 = GH & (w, Gamma) ++ GT) by skip;
+destruct H5 as (GH, H5); destruct H5 as (GT, H5); subst.
+apply t_letdia_get_LF with (L_w:=L_w \u \{w''}) 
+  (L_t:=L_t) (A:=A) (G:=GH++GT & (w', Gamma'++Gamma'')) (Gamma:=Gamma).
+skip. (* ok_Bg *)
+eapply IHHT with (w1:=w) (G0:=GH++GT & (w0, Gamma0)) (Gamma':=Gamma') (Gamma'':=Gamma''); eauto.
+subst; permut_simpl. skip. (* H0 + H1 *)
+permut_simpl.
+intros. 
+rewrite notin_union in H6; destruct H6.
+rewrite notin_singleton in H7.
+unfold open_var in *; unfold open_ctx in *.
+rewrite <- subst_ctx_comm.
+rewrite subst_order_irrelevant_free.
+eapply H with (G0:=(w'0, (v', A) :: nil) :: (GH ++ GT) & (w, Gamma)); eauto.
+permut_simpl. skip. (* H0 + H1 *)
+permut_simpl.
+simpl; auto.
+intro; subst; elim H7; auto.
+subst; permut_simpl.
+apply permut_sym. 
+skip. (*trans with H2 *)
+Admitted. (* "No more subgoals but non-instantiated existential variables" *)
+
+Lemma rename_w_preserv_types_new:
+forall G w Gamma A M G' w' Gamma'
+  (HT: G |= (w, Gamma) |- M ::: A)
+  (GG': permut G (G' & (w', Gamma'))),
+  G' |= (w, Gamma ++ Gamma') |- {{ fctx w // fctx w' }} M ::: A.
+intros;
+apply rename_w_preserv_types with (G := G) (w := w) (w':= w'); eauto.
+Qed.
+
+Lemma rename_w_preserv_types_old:
+forall G w Gamma A M G' w' Gamma'
+  (HT: G |= (w, Gamma) |- M ::: A)
+  (GG': permut G (G' & (w', Gamma'))),
+  G' |= (w', Gamma' ++ Gamma) |- {{ fctx w' // fctx w }} M ::: A.
+intros;
+apply rename_w_preserv_types with (G := G) (w := w) (w':= w'); eauto.
+Qed.
+
+Lemma rename_w_preserv_types_outer:
+forall G G0 w Gamma A M G' w' Gamma' w'' Gamma''
+  (HT: G |= (w, Gamma) |- M ::: A)
+  (GG: permut G (G0 & (w', Gamma') & (w'', Gamma'')))
+  (GG': permut G' (G0 & (w', Gamma' ++ Gamma''))),
+  G' |= (w, Gamma) |- {{ fctx w' // fctx w'' }} M ::: A.
+intros;
+eapply rename_w_preserv_types;
+eauto.
+Qed.
+
+Lemma Progress:
+forall G w M A
+  (H_lc_w: lc_w_LF M)
+  (H_lc_t: lc_t_LF M)
+  (HT: emptyEquiv G |= (w, nil) |- M ::: A),
+  value_LF M \/ exists N, (M, fctx w) |-> (N, fctx w).
+intros;
+remember (w, (@nil ty_LF)) as Ctx;
+generalize dependent Ctx;
+generalize dependent A;
+generalize dependent w;
+generalize dependent G.
+induction M; intros; eauto using value_LF;
+inversion HeqCtx; subst.
+(* hyp *)
+inversion HT; subst;
+rewrite Mem_nil_eq in HT0;
+contradiction.
+(* appl *)
+right; inversion HT; subst;
+inversion H_lc_t; subst;
+inversion H_lc_w; subst;
+edestruct IHM1 with (A := A0 ---> A); eauto;
+[ inversion H0; subst; inversion HT1; subst | 
+  destruct H0];
+eexists; constructor; eauto;
+inversion H2; inversion H3; subst; eauto.
+(* unbox & unbox_fetch *)
+right; inversion HT; subst;
+inversion H_lc_w; subst;
+inversion H_lc_t; subst.
+(* unbox *)
+edestruct IHM with (A := [*]A); eauto;
+[ inversion H0; subst; inversion HT0; subst |
+  destruct H0];
+eexists; constructor; eauto;
+inversion H3; inversion H4; subst; auto.
+(* unbox_fetch *)
+(* TODO: permut (G0 & (w0, Gamma)) (emptyEquiv G) --> Gamma = nil *)
+assert (Gamma = nil) by skip; subst. 
+destruct IHM with (A := [*]A) 
+                  (Ctx := (w0, (@nil ty_LF)))
+                  (G := G0 & (w0, nil))
+                  (w := w0); 
+eauto;
+(* TODO: emptyEqiv (G0 & (w0, nil)) = G0 & (w0, nil) by H6 *) 
+[ skip |
+  inversion H0; subst; inversion HT0; subst | 
+  destruct H0 ];
+eexists; constructor; eauto;
+inversion H3; inversion H4; subst; 
+eauto.
+(* here & get_here *)
+inversion HT; subst;
+inversion H_lc_w; subst;
+inversion H_lc_t; subst.
+(* here *)
+edestruct IHM; eauto;
+[ left; econstructor|
+  right; destruct H0; eexists];
+eauto using step_LF.
+(* get_here *)
+(* TODO: permut (G0 & (w0, Gamma)) (emptyEquiv G) --> Gamma = nil *)
+assert (Gamma = nil) by skip; subst;
+edestruct IHM with (A := A0) (G := G0 & (w0, nil)) (w:=w0); eauto;
+(* TODO: emptyEqiv (G0 & (w0, nil)) = G0 & (w0, nil) by H5 *) 
+[ skip | 
+  left; inversion H0; subst; inversion HT0; subst | 
+  right; destruct H0; eexists];
+econstructor; eauto using step_LF.
+(* letdia & letdia_get *)
+right; inversion HT; subst;
+inversion H_lc_w; subst;
+inversion H_lc_t; subst.
+(* letdia *)
+edestruct IHM1 with (A := <*>A0); eauto;
+[ inversion H0; subst; inversion HT1; subst |
+  destruct H0];
+eexists; constructor; eauto;
+try apply closed_t_succ; auto;
+inversion H5; inversion H7; subst; auto.
+(* letdia_get *)
+(* TODO: permut (G0 & (w0, Gamma)) (emptyEquiv G) --> Gamma = nil *)
+assert (Gamma = nil) by skip; subst.
+edestruct IHM1 with (G := G0 & (w, nil)) 
+                    (w := w0) 
+                    (Ctx := (w0, (@nil ty_LF)))
+                    (A := <*>A0); eauto;
+(* TODO: emptyEqiv (G0 & (w0, nil)) = G0 & (w0, nil) by H6 *) 
+[ skip |
+  inversion H0; subst; inversion HT1; subst |
+  destruct H0];
+eexists; constructor; eauto;
+try apply closed_t_succ; auto;
+inversion H5; inversion H8; subst; auto.
+Qed.
+
+
 Lemma Preservation:
 forall G M N A w
-  (HOk: ok_Bg ((w,nil)::emptyEquiv G) nil)
   (HT: emptyEquiv G |= (w, nil) |- M ::: A)
   (HS: (M, fctx w) |-> (N, fctx w)),
   emptyEquiv G |= (w, nil) |- N ::: A.
 intros;
+remember (w, (@nil (var * ty_LF))) as Ctx;
 remember (emptyEquiv G) as G';
-remember (w, (@nil ty_LF)) as Ctx;
 generalize dependent w;
 generalize dependent N;
 generalize dependent G;
@@ -1934,384 +882,67 @@ inversion HS; subst;
 try (inversion HeqCtx; subst);
 eauto using types_LF.
 (* appl_lam *)
-inversion HT1; subst.
-replace ([N//0 | fctx w ] [M0 | fctx w]) with 
-        (subst_list (N::nil) (length (@nil te_LF)) M0 (fctx w) (fctx w)) by auto.
-apply subst_t_preserv_types_inner with (Delta := A::nil).
-  simpl; split. rewrite emptyEquiv_stable. eauto. auto.
-  intros; rewrite Mem_cons_eq in H; destruct H.
-    subst; assumption.
-    rewrite Mem_nil_eq in H; contradiction.
-  simpl in *; assumption.
-  intros; repeat split; eauto.
+inversion HT1; subst;
+unfold open_var in *;
+assert (exists v, v \notin L) as HF by apply Fresh;
+destruct HF as (v_fresh);
+eapply subst_t_preserv_types_inner; eauto;
+(* TODO: Double emptyEquiv doesn't change more than single *)
+skip.
 (* unbox_box *)
-inversion HT; subst.
-assert (exists w0, w0 \notin L \u free_worlds_LF M0).
-  apply Fresh.
-destruct H as [w1].
-rewrite notin_union in H; destruct H.
-unfold open_ctx in *.
-eapply inv_subst_ctx_preserv_types with (w_fresh:=w1) (Gamma_fresh:=nil) (k:=0) (w_step:=w1); eauto.
-intros b; elim b; reflexivity.
-intros; repeat split; eauto.
-intros; repeat split; eauto. (* ?this should give contradiction? *)
-replace (w0, (@nil ty_LF)) with (w0, nil ++ (@nil ty_LF)).
-apply rename_ctx_preserv_types_old with (G':=(emptyEquiv G0 & (w0, nil))).
-skip.
-permut_simpl.
-apply HT0; auto.
-(* unbox_fetch_box *)
-inversion HT; subst.
-assert (exists w0, w0 \notin L \u free_worlds_LF M0).
-  apply Fresh.
-destruct H0 as [w1].
-rewrite notin_union in H0; destruct H0.
-unfold open_ctx in *.
-eapply inv_subst_ctx_preserv_types with (w_fresh:=w1) (w_step :=w1) (Gamma_fresh:=nil) (k:=0); eauto.
-intros b; elim b; reflexivity.
-intros; repeat split; eauto.
-intros; repeat split; eauto.
-replace (w0, (@nil ty_LF)) with (w0, nil ++ (@nil ty_LF)).
-apply rename_ctx_preserv_types_old with (G':=(emptyEquiv G0 & (w0, nil))).
-skip.
-permut_simpl.
-apply BackgroundSubsetImpl with (G:= G & (w0,nil) & (w,Gamma)).
-  rew_app in *; apply HT0; auto.
-  exists (@nil Context_LF); permut_simpl; assumption.
-  auto.
-(* unbox_fetch *)
-apply t_unbox_fetch_LF with (G:=G) (Gamma:=Gamma).
-assert (Gamma = nil).
-apply emptyEquiv_nil with (G:=G0) (G':=G & (w, Gamma)) (w:=w).
-  apply permut_sym; assumption.
-  apply Mem_last.
-subst.
-apply IHHT with (G0:=G & (w0, nil)) (w1 := w); auto.
-apply ok_Bg_permut with (G:=(w0, nil)::emptyEquiv G0).
-apply permut_trans with (l2:=(w0,nil) :: G & (w, nil)); permut_simpl.
-apply permut_sym; assumption.
-assumption.
-
-rewrite emptyEquiv_last with (G':=G).
-reflexivity.
-apply emptyEquiv_inv with (w:=w).
-apply emptyEquiv_empty with (G:=G0).
-  apply permut_sym; assumption.
-assumption.
-(* get_here *)
-apply t_get_here_LF with (G:=G) (Gamma:=Gamma); auto.
-assert (Gamma = nil).
-apply emptyEquiv_nil with (G:=G0) (G':=G & (w, Gamma)) (w:=w).
-  apply permut_sym; assumption.
-  apply Mem_last.
-subst.
-apply IHHT with (G0:=G & (w0,nil)) (w1:=w); auto.
-
-apply ok_Bg_permut with (G:=(w0, nil)::emptyEquiv G0).
-apply permut_trans with (l2:=(w0,nil) :: G & (w, nil)); permut_simpl.
-apply permut_sym; assumption.
-assumption.
-
-rewrite emptyEquiv_last with (G':=G).
-reflexivity.
-apply emptyEquiv_inv with (w:=w).
-apply emptyEquiv_empty with (G:=G0).
-  apply permut_sym; assumption.
-(* letdia + (here | get_here ) *)
-inversion HT; subst.
-(* letdia_here *)
-assert (exists w1, w1 \notin L \u free_worlds_LF N) by apply Fresh.
-destruct H0 as [w1];
-apply notin_union in H0;
-destruct H0.
-replace ([M0 // 0 | fctx w0] [N ^^ [fctx w0 | fctx w0] | fctx w0])
-   with (subst_list (M0::nil) (length (@nil te_LF)) (N ^^ [fctx w0 | fctx w0]) (fctx w0) (fctx w0)) by auto.
-eapply subst_t_preserv_types_inner with (Delta:=A::nil). 
-  simpl; split; auto;
-  rewrite emptyEquiv_stable;
-  assumption.
-intros. rewrite Mem_cons_eq in H3; destruct H3.
-  subst; assumption.
-  rewrite Mem_nil_eq in H3; contradiction.
-simpl in *; assumption.
-unfold open_ctx in *.
-  replace (w0, (nil & A)) with (w0, (A::nil) ++ (@nil ty_LF)).
-  eapply inv_subst_ctx_preserv_types_new; eauto.
-  apply rename_ctx_preserv_types_new with (G':=(emptyEquiv G0 & (w1, A::nil))).
-  skip.
-  permut_simpl.
-  apply BackgroundSubsetImpl with (G:= (w1, A::nil) :: emptyEquiv G0).
-  apply HT2; auto.
-  eexists; permut_simpl.
-  rew_app; reflexivity.
-(* letdia__get_here *)
-assert (exists w1, w1 \notin L \u free_worlds_LF N) by apply Fresh.
-destruct H0 as [w1];
-apply notin_union in H0;
-destruct H0.
-assert (Gamma = nil).
-apply emptyEquiv_nil with (G:=G0) (G':=G & (w, Gamma)) (w:=w).
-  apply permut_sym; assumption.
-  apply Mem_last.
-subst.
-assert (w <> w0).
-  eapply unique_worlds; eauto.
-replace ([M0 // 0 | fctx w] [N ^^ [fctx w | fctx w0] | fctx w0])
-   with (subst_list (M0::nil) (length (@nil te_LF)) (N ^^ [fctx w | fctx w0]) (fctx w) (fctx w0)) by auto.
-apply subst_t_preserv_types with (G0:=G) (Delta:=A::nil) (G_min:= G & (w0, nil)) (G_HT:= G & (w, nil & A)) (Gamma_subst:= nil) (Gamma_HT := nil) .
-  simpl; split; auto.
-  rewrite emptyEquiv_last with (G':=G).
-    assumption.
-  apply emptyEquiv_inv with (w:=w).
-  rewrite emptyEquiv_empty with (G:= emptyEquiv G0).
-    reflexivity.
-    rewrite emptyEquiv_stable.
-    apply permut_sym; assumption.
-intros. rewrite Mem_cons_eq in H5; destruct H5.
-  subst; assumption.
-  rewrite Mem_nil_eq in H5; contradiction.
-  intro; contradiction.
-  intro; repeat split; auto; apply permut_sym; auto.
-  simpl in *. case_if. apply ok_Bg_permut with (G':=(w,nil)::G) in HOk.
-  apply ok_Bg_permut with (G:=(w,nil & A)::G).
-  permut_simpl.
-  simpl in *; assumption.
-  apply permut_trans with (l2:=G & (w, nil)); try apply permut_sym; permut_simpl; eauto.
-  unfold open_ctx in *.
-  apply inv_subst_ctx_preserv_types_outer with (G0:=G) (G:=G & (w, A::nil)) (w':=w1) (Gamma:=nil) (Gamma':=A::nil) (k:=0).
-  assumption.
-  permut_simpl.
-  apply rename_ctx_preserv_types_outer with (G':=(emptyEquiv G0 & (w1, A::nil)))
-    (G := G) (Gamma := nil).
-  skip.
-  permut_simpl; apply permut_sym; assumption.
-  permut_simpl.
-  apply BackgroundSubsetImpl with (G:= (w1, A :: nil) :: emptyEquiv G0).
-  apply HT2; auto.
-  exists (@nil Context_LF); permut_simpl; assumption.
-(* letdia_get + ( here | get_here) *)
-inversion HT; subst.
-(* letdia_get__here *)
-assert (exists w1, w1 \notin L \u free_worlds_LF N).
-  apply Fresh.
-destruct H1 as [w2].
-apply notin_union in H1;
-destruct H1.
-assert (Gamma = nil).
-apply emptyEquiv_nil with (G:=G1) (G':=G & (w, Gamma)) (w:=w).
-  apply permut_sym; assumption.
-  apply Mem_last.
-subst.
-replace ([M0 // 0 | fctx w] [N ^^ [fctx w | fctx w0] | fctx w0])
-   with (subst_list (M0::nil) (length (@nil te_LF)) (N ^^ [fctx w | fctx w0]) (fctx w) (fctx w0)) by auto.
-apply subst_t_preserv_types with (G0:=G) (Delta:=A::nil) (G_min:= G & (w0, nil)) (G_HT:= G & (w, nil & A)) (Gamma_subst:= nil) (Gamma_HT:=nil).
-  simpl; split; auto.
-  rewrite emptyEquiv_last with (G':=G).
-    assumption.
-  apply emptyEquiv_inv with (w:=w).
-  rewrite emptyEquiv_empty with (G:= emptyEquiv G1).
-    reflexivity.
-    rewrite emptyEquiv_stable.
-    apply permut_sym; assumption.
-intros. rewrite Mem_cons_eq in H4; destruct H4.
-  subst; assumption.
-  rewrite Mem_nil_eq in H4; contradiction.
-  intro. absurd (w = w0). eapply unique_worlds; eauto.
-  assumption.
-  intro; repeat split; auto; apply permut_sym; auto.
-
-  simpl in *. case_if. apply ok_Bg_permut with (G':=(w,nil)::G) in HOk.
-  apply ok_Bg_permut with (G:=(w,nil & A)::G).
-  permut_simpl.
-  simpl in *; assumption.
-  apply permut_trans with (l2:=G & (w, nil)); try apply permut_sym; permut_simpl; eauto.
-
-  unfold open_ctx in *.
-  apply inv_subst_ctx_preserv_types_outer with (G0:=G) (G:=G & (w, A::nil)) (w':=w2) (Gamma:=nil) (Gamma':=A::nil) (k:=0).
-  assumption.
-  permut_simpl.
-  apply rename_ctx_preserv_types_outer with (G':=(emptyEquiv G1 & (w2, A::nil)))
-    (G := G) (Gamma := nil).
-  skip.
-  permut_simpl; apply permut_sym; assumption.
-  permut_simpl.
-  apply BackgroundSubsetImpl with (G:= (w2, A :: nil) :: G & (w,nil)).
-  replace (fctx w0) with (fctx (fst (w0, (@nil ty_LF)))).
-  apply HT2; auto.
-  simpl; reflexivity.
-  exists (@nil Context_LF); permut_simpl; assumption.
-(* letdia_get_get_here *)
-assert (Gamma = nil).
-apply emptyEquiv_nil with (G:=G1) (G':=G & (w, Gamma)) (w:=w).
-  apply permut_sym; assumption.
-  apply Mem_last.
-subst.
-assert (Gamma0 = nil).
-apply emptyEquiv_nil with (G:=G & (w0, nil)) (G':=G0 & (w1, Gamma0)) (w:=w1).
-  rewrite emptyEquiv_last with (G':=G).
-  apply permut_sym; assumption.
-  apply emptyEquiv_inv with (w:=w).
-  apply emptyEquiv_empty with (G:=G1).
-  apply permut_sym; assumption.
-  apply Mem_last.
-subst.
-assert (exists w1, w1 \notin L \u free_worlds_LF N).
-  apply Fresh.
-destruct H1 as [w2].
-apply notin_union in H1;
-destruct H1.
-replace ([M0 // 0 | fctx w1] [N ^^ [fctx w1 | fctx w0] | fctx w0])
-   with (subst_list (M0::nil) (length (@nil te_LF)) (N ^^ [fctx w1 | fctx w0]) (fctx w1) (fctx w0)) by auto.
-destruct (eq_var_LF_dec w0 w1).
-(* = *)
-subst.
-assert (permut (G0 & (w1, nil) ++ nil) (G & (w1, nil) ++ nil)).
-rew_app; assumption.
-apply permut_inv in H4; rew_app in H4.
-eapply subst_t_preserv_types_inner with (Delta:=A::nil). 
-simpl; split; auto.
-rewrite emptyEquiv_stable; 
-apply BackgroundSubsetImpl with (G:=G0 & (w,nil)).
-assumption.
-exists (@nil Context_LF).
-rew_app.
-apply permut_trans with (l2:=G&(w,nil));
-permut_simpl; assumption.
-intros. rewrite Mem_cons_eq in H6; destruct H6.
-  subst; assumption.
-  rewrite Mem_nil_eq in H6; contradiction.
-assumption.
-unfold open_ctx in *.
-replace (w1, (nil & A)) with (w1, (A::nil) ++ (@nil ty_LF)).
-  apply inv_subst_ctx_preserv_types_new with (w':=w2) (k:=0). 
-  assumption.
-apply rename_ctx_preserv_types_new with (G':=(emptyEquiv G1 & (w2, A::nil))).
-skip.
-permut_simpl.
-  apply BackgroundSubsetImpl with (G:= (w2, A :: nil) :: G & (w, nil)).
-  apply HT2.
-  assumption.
-  exists (@nil Context_LF); permut_simpl; assumption.
-  auto.
-(* <> *)
-assert (exists GH, exists GT, G = GH & (w1, nil) ++ GT). 
-apply permut_split_neq with (G := G0) (G' := nil) (elem' := (w0, nil)).
-intro; inversion H4; subst; elim n; reflexivity.
-rew_app; assumption.
-destruct H4 as (GH).
-destruct H4 as (GT).
-subst G.
-assert (permut (G0++nil) (GH ++ GT & (w0,nil)++nil )).
-  apply permut_inv with (elem:=(w1,nil)); rew_app.
-  apply permut_trans with (l2:=(GH & (w1, nil) ++ GT) & (w0, nil)).
-    assumption.
-    permut_simpl.
-rew_app in H4.
-assert (w <> w0).
-eapply unique_worlds with (G':=(GH & (w1, nil) ++ GT) & (w0, nil));
+inversion HT; subst;
+assert (exists v, v \notin L \u (free_worlds_LF M0)) as HF by apply Fresh;
+destruct HF as (w_fresh);
+unfold open_ctx in *;
+replace ({{fctx w0 // bctx 0}}M0)
+  with ({{fctx w0 // fctx w_fresh}} {{fctx w_fresh // bctx 0}}M0)
+  by (rewrite subst_ctx_neutral_free; auto);
+replace (@nil (var * ty_LF)) with (nil ++ (@nil (var * ty_LF))); eauto;
+apply rename_w_preserv_types_old with (G := emptyEquiv G0 & (w0, nil));
 eauto.
-assert (permut (emptyEquiv G1 & (w0, nil)) (G0 & (w1,nil) &(w,nil))).
-  apply permut_trans with (l2:=GH & (w1, nil) ++ GT & (w,nil)  & (w0, nil) ).
-  permut_simpl. rew_app in H0. rew_app. apply permut_sym; assumption.
-  permut_simpl; apply permut_sym; assumption.
-assert (exists GH', exists GT', G0 & (w1,nil) = GH' & (w0,nil) ++ GT').
-apply permut_split_neq with (G := emptyEquiv G1) (G' := nil) (elem' := (w, nil)).
-intro; inversion H9; subst; elim H6; reflexivity.
-rew_app in *; assumption.
-destruct H9 as (GH').
-destruct H9 as (GT').
-assert (exists GH'', exists GT'', G0 = GH'' & (w0, nil) ++ GT'').
-apply permut_split_neq with (G := GH') (G' := GT') (elem' := (w1, nil)).
-intro; inversion H10; subst; elim n; reflexivity.
-rewrite <- H9; permut_simpl.
-destruct H10 as (GH'').
-destruct H10 as (GT'').
-subst G0.
-assert (permut (emptyEquiv G1 ++ nil) ((GH'' ++ GT'') & (w, nil) & (w1, nil))).
-apply permut_inv with (elem := (w0,nil)).
-rew_app in *.
-apply permut_trans with (l2:=(GH'' ++ (w0, nil) :: GT'' ++ (w1, nil) :: (w, nil) :: nil)).
-assumption. permut_simpl.
-apply subst_t_preserv_types with (G0 := GH''++GT'' & (w, nil)) 
-  (Delta:=A::nil) (G_min:= GH'' ++ GT'' & (w, nil) & (w0, nil)) (G_HT:= (GH'' ++ GT'' & (w, nil)) & (w1, nil & A)) (Gamma_subst:= nil) (Gamma_HT:=nil).
-  simpl; split; auto.
-  rewrite emptyEquiv_inv with (w:=w1) (G':=(GH'' ++ GT'' & (w, nil) & (w0, nil))).
-  apply BackgroundSubsetImpl with (G:=(GH'' & (w0, nil) ++ GT'') & (w, nil)).
-  apply HT0.
-  exists (@nil Context_LF); permut_simpl.
-  apply emptyEquiv_last.
-  replace ( GH'' ++ GT'' & (w, nil) & (w0, nil) ) with (( GH'' ++ GT'' & (w, nil)) & (w0, nil)).
-  apply emptyEquiv_last.
-  apply emptyEquiv_inv with (w:=w1).
-  apply emptyEquiv_empty with (G:=G1). 
-  rew_app in *. assumption.
-  rew_app; reflexivity.
-intros. rewrite Mem_cons_eq in H11; destruct H11.
-  subst; assumption.
-  rewrite Mem_nil_eq in H11; contradiction.
-intro neq; symmetry in neq. subst; elim n. reflexivity. 
-intro; repeat split; eauto; permut_simpl. rew_app in *; assumption.
+(* unbox_fetch_box *)
+inversion HT; subst;
+assert (exists v, v \notin L \u (free_worlds_LF M0)) as HF by apply Fresh;
+destruct HF as (w_fresh);
+unfold open_ctx in *;
+replace ({{fctx w0 // bctx 0}}M0)
+  with ({{fctx w0 // fctx w_fresh}} {{fctx w_fresh // bctx 0}}M0)
+  by (rewrite subst_ctx_neutral_free; auto);
+replace (@nil (var * ty_LF)) with (nil ++ (@nil (var * ty_LF))); eauto;
+apply rename_w_preserv_types_old with (G := G & (w0, nil) & (w, Gamma));
+try permut_simpl;
+eauto.
+(* unbox_fetch *)
+econstructor; eauto;
+(* TODO: permut (G & (w, Gamma)) (emptyEquiv G0) -> Gamma = nil *)
+assert (Gamma = nil) by skip; subst;
+eapply IHHT with (G0:=G & (w0, nil)); eauto;
+(* TODO: by H, G contains no Gammas <> nil, so taking emptyEquiv doesn't change anything *)
+skip.
+(* get_here *)
+econstructor; eauto;
+(* TODO: permut (G & (w, Gamma)) (emptyEquiv G0) -> Gamma = nil *)
+assert (Gamma = nil) by skip; subst;
+eapply IHHT with (G0:=G & (w0, nil)); eauto;
+(* TODO: by H, G contains no Gammas <> nil, so taking emptyEquiv doesn't change anything *)
+skip.
+(* letdia + (here | get_here ) *)
+assert (exists w1, w1 \notin L_w \u free_worlds_LF N) as HF by apply Fresh;
+assert (exists v1, v1 \notin L_w) as HF2 by apply Fresh;
+destruct HF as (w_fresh); destruct HF2 as (v_fresh);
+inversion HT; subst. 
+(* letdia here *)
+apply subst_t_preserv_types_inner with (L:=L_t) (A:=A); auto.
+intros.
+unfold open_ctx in *; unfold open_var in *.
+rewrite <- subst_ctx_neutral_free with (w0:=w_fresh);
+eauto; rewrite <- subst_ctx_neutral_bound with (n:=0).
+eapply rename_w_preserv_types_new.
+[ | skip ]. (* emptyEquiv (emptyEquiv G) = emptyEquiv G + HT0 *)
+intros. apply 
 
-simpl in *. 
-case_if.
-rewrite ok_Bg_emptyEquiv.
-apply ok_Bg_permut with (G:=emptyEquiv G1).
-apply permut_trans with (l2:=(GH'' ++ GT'') & (w, nil) & (w1, nil)).
-rew_app in *; assumption.
-rewrite emptyEquiv_last with (G':= (GH'' ++ GT'') & (w, nil)).
-permut_simpl.
-assert ((GH'' ++ GT'') & (w, nil) & (w1, nil) = emptyEquiv ((GH'' ++ GT'') & (w, nil) & (w1, nil))).
-symmetry; apply emptyEquiv_empty with (G:=G1).
-rew_app in *; assumption.
-assert (permut ((GH'' ++ GT'') & (w, nil) & (w1, nil)) (emptyEquiv ((GH'' ++ GT'') & (w, nil) & (w1, nil)))).
-rewrite <- H12; permut_simpl.
-assert (permut (emptyEquiv (GH'' ++ GT'' & (w, nil)) ++ nil) ((GH'' ++ GT'' & (w, nil))++nil)).
-apply permut_inv with (elem := (w1, nil)).
-apply permut_sym.
-rewrite emptyEquiv_last with (G':=emptyEquiv ((GH'' ++ GT'') & (w, nil))) in H13.
-rew_app in *; assumption.
-reflexivity.
-rew_app.
-apply emptyEquiv_empty with (G:=GH'' ++ GT'' & (w, nil)).
-rew_app in *; assumption.
-assumption.
-
-unfold open_ctx in *.
-  apply inv_subst_ctx_preserv_types_outer with (w':=w2) (Gamma':=A::nil) (Gamma:=nil) (G0:=(GH'' ++ GT'' & (w, nil))).
-  assumption.
-  permut_simpl.
-  replace (fctx w0) with (fctx (fst (w0, (@nil ty_LF)))).
-  apply rename_ctx_preserv_types_outer with (G':=(emptyEquiv G1 & (w2, A::nil))) (Gamma:=nil) (G:=GH''++GT'' & (w,nil)).
-  skip.
-  permut_simpl; rew_app in H10.
-  apply permut_trans with (l2:=GH'' ++ GT'' ++ (w, nil) :: (w1, nil) :: nil).
-    assumption.
-    permut_simpl.
-  permut_simpl.
-  apply BackgroundSubsetImpl with (G:=(w2, A :: nil) :: (GH & (w1, nil) ++ GT) & (w, nil)).
-  apply HT2 with (w':=w2); auto.
-  exists (@nil Context_LF). permut_simpl.
-  rew_app in *; assumption.
-  simpl; reflexivity.
-(* letdia_get *)
-apply t_letdia_get_LF with (L:=L)(A:=A) (G:=G) (Gamma:=Gamma); auto.
-assert (Gamma = nil).
-apply emptyEquiv_nil with (G:=G1) (G':=G & (w, Gamma)) (w:=w).
-  apply permut_sym; assumption.
-  apply Mem_last.
-subst.
-apply IHHT with (G0:=G & (w0,nil)) (w1:=w); auto.
-
-apply ok_Bg_permut with (G:=(w0, nil)::emptyEquiv G1).
-apply permut_trans with (l2:=(w0,nil) :: G & (w, nil)); permut_simpl.
-apply permut_sym; assumption.
-assumption.
-
-rewrite emptyEquiv_last with (G':=G).
-reflexivity.
-apply emptyEquiv_inv with (w:=w).
-apply emptyEquiv_empty with (G:=G1).
-apply permut_sym; assumption.
+skip.
+skip.
 Qed.
 
 End Lemmas.
